automated some proofs

TaskinBA/Complement_DPDA.thy
@@ -14,7 +14,8 @@ qed
 
 context dpda begin
 
-definition "end_check_final_states \<equiv> P ` final_states M"
+definition end_check_final_states :: "'q st_primed set" where
+  "end_check_final_states \<equiv> P ` final_states M"
 
 fun end_check_trans_fun :: "'q st_primed \<Rightarrow> 'a input_with_marker \<Rightarrow> 's \<Rightarrow> ('q st_primed \<times> 's list) set" where
   "end_check_trans_fun (N q) (Input a) Z = (\<lambda>(p, \<alpha>). (N p, \<alpha>)) ` (trans_fun M q (Input a) Z)"
@@ -30,39 +31,27 @@ definition end_check_dpda :: "('q st_primed, 'a input_with_marker, 's) pda" wher
                       final_states = end_check_final_states, trans_fun = end_check_trans_fun, eps_fun = end_check_eps_fun \<rparr>"
 
 lemma end_check_card_trans_N: "card (end_check_trans_fun (N q) a Z) = card (trans_fun M q a Z)"
-proof -
-  have inj_on_N: "inj_on (\<lambda>(p, \<alpha>). (N p, \<alpha>)) (trans_fun M q a Z)"
-    by (auto simp: inj_on_def)
-  have inj_on_P: "inj_on (\<lambda>(p, \<alpha>). (P p, \<alpha>)) (trans_fun M q a Z)"
-    by (auto simp: inj_on_def)
-  show ?thesis
-  using card_image[OF inj_on_N] card_image[OF inj_on_P]
-  by (induction "N q" a Z rule: end_check_trans_fun.induct) auto
-qed
+  apply (induction "N q" a Z rule: end_check_trans_fun.induct)
+   apply (rule sym, rule bij_betw_same_card[where ?f = "\<lambda>(p, \<alpha>). (N p, \<alpha>)"])
+   defer
+   apply (rule sym, rule bij_betw_same_card[where ?f = "\<lambda>(p, \<alpha>). (P p, \<alpha>)"])
+   apply (auto simp: bij_betw_def inj_on_def)
+  done
 
 lemma end_check_card_trans_P: "card (end_check_trans_fun (P q) a Z) = card (trans_fun M q a Z)"
-proof -
-  have inj_on_P: "inj_on (\<lambda>(p, \<alpha>). (P p, \<alpha>)) (trans_fun M q a Z)"
-    by (auto simp: inj_on_def)
-  show ?thesis
-  using card_image[OF inj_on_P] by simp
-qed
+  apply (rule sym, rule bij_betw_same_card[where ?f = "\<lambda>(p, \<alpha>). (P p, \<alpha>)"])
+    apply (auto simp: bij_betw_def inj_on_def)
+  done
 
 lemma end_check_card_eps_N: "card (end_check_eps_fun (N q) Z) = card (eps_fun M q Z)"
-proof -
-  have inj_on_N: "inj_on (\<lambda>(p, \<alpha>). (N p, \<alpha>)) (eps_fun M q Z)"
-    by (auto simp: inj_on_def)
-  show ?thesis
-    using card_image[OF inj_on_N] by simp
-qed
+  apply (rule sym, rule bij_betw_same_card[where ?f = "\<lambda>(p, \<alpha>). (N p, \<alpha>)"])
+    apply (auto simp: bij_betw_def inj_on_def)
+  done
 
 lemma end_check_card_eps_P: "card (end_check_eps_fun (P q) Z) = card (eps_fun M q Z)"
-proof -
-  have inj_on_P: "inj_on (\<lambda>(p, \<alpha>). (P p, \<alpha>)) (eps_fun M q Z)"
-    by (auto simp: inj_on_def)
-  show ?thesis
-    using card_image[OF inj_on_P] by simp
-qed
+  apply (rule sym, rule bij_betw_same_card[where ?f = "\<lambda>(p, \<alpha>). (P p, \<alpha>)"])
+    apply (auto simp: bij_betw_def inj_on_def)
+  done
 
 lemma dpda_end_check: "dpda end_check_dpda"
 proof (standard, goal_cases)
@@ -70,13 +59,13 @@ proof (standard, goal_cases)
   have "finite (end_check_trans_fun p x z)"
     by (induction p x z rule: end_check_trans_fun.induct) (auto simp: finite_trans)
   then show ?case
-    unfolding end_check_dpda_def by simp
+    by (simp add: end_check_dpda_def)
 next
   case (2 p z)
   have "finite (end_check_eps_fun p z)"
     by (induction p z rule: end_check_eps_fun.induct) (auto simp: finite_eps)
   then show ?case
-    unfolding end_check_dpda_def by simp
+    by (simp add: end_check_dpda_def)
 next
   case (3 q a Z)
   then show ?case 
@@ -85,165 +74,56 @@ next
 next
   case (4 q \<alpha> p a)
   hence "(q, \<alpha>) \<in> end_check_trans_fun p a (init_symbol M)"
-    unfolding end_check_dpda_def by simp
+    by (simp add: end_check_dpda_def)
   hence "\<exists>\<alpha>'. \<alpha> = \<alpha>' @ [init_symbol M]"
     by (induction p a "init_symbol M" rule: end_check_trans_fun.induct) (auto simp: init_trans)
   thus ?case
-    unfolding end_check_dpda_def by simp
+    by (simp add: end_check_dpda_def)
 next
   case (5 q \<alpha> p)
   hence "(q, \<alpha>) \<in> end_check_eps_fun p (init_symbol M)"
-    unfolding end_check_dpda_def by simp
+    by (simp add: end_check_dpda_def)
   hence "\<exists>\<alpha>'. \<alpha> = \<alpha>' @ [init_symbol M]"
     by (induction p "init_symbol M" rule: end_check_eps_fun.induct) (auto simp: init_eps)
   thus ?case
-    unfolding end_check_dpda_def by simp
+    by (simp add: end_check_dpda_def)
 qed
 
 lemma pda_end_check: "pda end_check_dpda"
   using dpda_def dpda_end_check by auto
 
-lemma end_check_dpda_trans_N: 
-"(p\<^sub>2, \<beta>) \<in> trans_fun M p\<^sub>1 (Input a) Z \<longleftrightarrow> (N p\<^sub>2, \<beta>) \<in> trans_fun end_check_dpda (N p\<^sub>1) (Input a) Z"
-(is "?l \<longleftrightarrow> ?r")
-proof 
-  show "?l \<Longrightarrow> ?r" by (auto simp: end_check_dpda_def)
-next
-  have "(N p\<^sub>2, \<beta>) \<in> end_check_trans_fun (N p\<^sub>1) (Input a) Z \<Longrightarrow> (p\<^sub>2, \<beta>) \<in> trans_fun M p\<^sub>1 (Input a) Z"
-    by (induction "N p\<^sub>1" "Input a" Z rule: end_check_trans_fun.induct) auto
-  thus "?r \<Longrightarrow> ?l"
-    by (simp add: end_check_dpda_def)
-qed
-
-lemma end_check_dpda_eps_N: 
-"(p\<^sub>2, \<beta>) \<in> eps_fun M p\<^sub>1 Z \<longleftrightarrow> (N p\<^sub>2, \<beta>) \<in> eps_fun end_check_dpda (N p\<^sub>1) Z"
-(is "?l \<longleftrightarrow> ?r")
-proof 
-  show "?l \<Longrightarrow> ?r" by (auto simp: end_check_dpda_def)
-next
-  have "(N p\<^sub>2, \<beta>) \<in> end_check_eps_fun (N p\<^sub>1) Z \<Longrightarrow> (p\<^sub>2, \<beta>) \<in> eps_fun M p\<^sub>1 Z"
-    by (induction "N p\<^sub>1" Z rule: end_check_eps_fun.induct) auto
-  thus "?r \<Longrightarrow> ?l"
-    by (simp add: end_check_dpda_def)
-qed
-
-lemma end_check_dpda_trans_marker_N:
-"(p\<^sub>2, \<beta>) \<in> trans_fun M p\<^sub>1 End_marker Z \<longleftrightarrow> (P p\<^sub>2, \<beta>) \<in> trans_fun end_check_dpda (N p\<^sub>1) End_marker Z" (is "?l \<longleftrightarrow> ?r")
-proof
-  show "?l \<Longrightarrow> ?r" by (auto simp: end_check_dpda_def)
-next
-  have "(P p\<^sub>2, \<beta>) \<in> end_check_trans_fun (N p\<^sub>1) End_marker Z \<Longrightarrow> (p\<^sub>2, \<beta>) \<in> trans_fun M p\<^sub>1 End_marker Z"
-    by (induction "N p\<^sub>1" "End_marker :: 'a input_with_marker" Z rule: end_check_trans_fun.induct) auto
-  thus "?r \<Longrightarrow> ?l"
-    by (simp add: end_check_dpda_def)
-qed
-
-lemma end_check_dpda_eps_P:
-"(p\<^sub>2, \<beta>) \<in> eps_fun M p\<^sub>1 Z \<longleftrightarrow> (P p\<^sub>2, \<beta>) \<in> eps_fun end_check_dpda (P p\<^sub>1) Z" (is "?l \<longleftrightarrow> ?r")
-proof
-  show "?l \<Longrightarrow> ?r" by (auto simp: end_check_dpda_def)
-next
-  have "(P p\<^sub>2, \<beta>) \<in> end_check_eps_fun (P p\<^sub>1) Z \<Longrightarrow> (p\<^sub>2, \<beta>) \<in> eps_fun M p\<^sub>1 Z"
-    by (induction "P p\<^sub>1" Z rule: end_check_eps_fun.induct) auto
-  thus "?r \<Longrightarrow> ?l"
-    by (simp add: end_check_dpda_def)
-qed
-
-lemma end_check_dpda_trans_P:
-"(p\<^sub>2, \<beta>) \<in> trans_fun M p\<^sub>1 a Z \<longleftrightarrow> (P p\<^sub>2, \<beta>) \<in> trans_fun end_check_dpda (P p\<^sub>1) a Z" (is "?l \<longleftrightarrow> ?r")
-proof
-  show "?l \<Longrightarrow> ?r" by (auto simp: end_check_dpda_def)
-next
-  have "(P p\<^sub>2, \<beta>) \<in> end_check_trans_fun (P p\<^sub>1) a Z \<Longrightarrow> (p\<^sub>2, \<beta>) \<in> trans_fun M p\<^sub>1 a Z"
-    by (induction "P p\<^sub>1" a Z rule: end_check_trans_fun.induct) auto
-  thus "?r \<Longrightarrow> ?l"
-    by (simp add: end_check_dpda_def)
-qed
-
 lemma end_check_dpda_input_step\<^sub>1:
   "pda.step\<^sub>1 M (p\<^sub>1, map Input w\<^sub>1, \<alpha>\<^sub>1) (p\<^sub>2, w\<^sub>2, \<alpha>\<^sub>2) \<longleftrightarrow>
-    pda.step\<^sub>1 end_check_dpda (N p\<^sub>1, map Input w\<^sub>1, \<alpha>\<^sub>1) (N p\<^sub>2, w\<^sub>2, \<alpha>\<^sub>2)" (is "?l \<longleftrightarrow> ?r")
-proof
-  assume ?l
-  then obtain Z \<alpha> where \<alpha>1_def: "\<alpha>\<^sub>1 = Z#\<alpha>" and rule:
-       "(\<exists>\<beta>. w\<^sub>2 = map Input w\<^sub>1 \<and> \<alpha>\<^sub>2 = \<beta> @ \<alpha> \<and> (p\<^sub>2, \<beta>) \<in> eps_fun M p\<^sub>1 Z) \<or>
-          (\<exists>a \<beta>. map Input w\<^sub>1 = Input a # w\<^sub>2 \<and> \<alpha>\<^sub>2 = \<beta> @ \<alpha> \<and> (p\<^sub>2, \<beta>) \<in> trans_fun M p\<^sub>1 (Input a) Z)"
-    using step\<^sub>1_rule_ext by auto
-  from rule have "(\<exists>\<beta>. w\<^sub>2 = map Input w\<^sub>1 \<and> \<alpha>\<^sub>2 = \<beta> @ \<alpha> \<and> (N p\<^sub>2, \<beta>) \<in> eps_fun end_check_dpda (N p\<^sub>1) Z) \<or>
-     (\<exists>a \<beta>. map Input w\<^sub>1 = Input a # w\<^sub>2 \<and> \<alpha>\<^sub>2 = \<beta> @ \<alpha> \<and> (N p\<^sub>2, \<beta>) \<in> trans_fun end_check_dpda (N p\<^sub>1) (Input a) Z)"
-    using end_check_dpda_trans_N end_check_dpda_eps_N by simp
-  with \<alpha>1_def show ?r
-    using pda.step\<^sub>1_rule[OF pda_end_check] by auto
-next
-  assume ?r
-  then obtain Z \<alpha> where \<alpha>1_def: "\<alpha>\<^sub>1 = Z#\<alpha>" and rule:
-       "(\<exists>\<beta>. w\<^sub>2 = map Input w\<^sub>1 \<and> \<alpha>\<^sub>2 = \<beta> @ \<alpha> \<and> (N p\<^sub>2, \<beta>) \<in> eps_fun end_check_dpda (N p\<^sub>1) Z) \<or>
-          (\<exists>a \<beta>. map Input w\<^sub>1 = Input a # w\<^sub>2 \<and> \<alpha>\<^sub>2 = \<beta> @ \<alpha> \<and> (N p\<^sub>2, \<beta>) \<in> trans_fun end_check_dpda (N p\<^sub>1) (Input a) Z)"
-    using pda.step\<^sub>1_rule_ext[OF pda_end_check] by auto
-  from rule have "(\<exists>\<beta>. w\<^sub>2 = map Input w\<^sub>1 \<and> \<alpha>\<^sub>2 = \<beta> @ \<alpha> \<and> (p\<^sub>2, \<beta>) \<in> eps_fun M p\<^sub>1 Z) \<or>
-     (\<exists>a \<beta>. map Input w\<^sub>1 = Input a # w\<^sub>2 \<and> \<alpha>\<^sub>2 = \<beta> @ \<alpha> \<and> (p\<^sub>2, \<beta>) \<in> trans_fun M p\<^sub>1 (Input a) Z)"
-    using end_check_dpda_trans_N end_check_dpda_eps_N by simp
-  with \<alpha>1_def show ?l
-    using step\<^sub>1_rule by auto
-qed
+    pda.step\<^sub>1 end_check_dpda (N p\<^sub>1, map Input w\<^sub>1, \<alpha>\<^sub>1) (N p\<^sub>2, w\<^sub>2, \<alpha>\<^sub>2)"
+by (use step\<^sub>1_rule_ext end_check_dpda_def pda.step\<^sub>1_rule_ext[OF pda_end_check] in auto)
 
 lemma end_check_dpda_marker_step\<^sub>1:
   "pda.step\<^sub>1 M (p\<^sub>1, End_marker#w, \<alpha>\<^sub>1) (p\<^sub>2, w, \<alpha>\<^sub>2) \<longleftrightarrow>
-    pda.step\<^sub>1 end_check_dpda (N p\<^sub>1, End_marker#w, \<alpha>\<^sub>1) (P p\<^sub>2, w, \<alpha>\<^sub>2)" (is "?l \<longleftrightarrow> ?r")
-proof
-  assume ?l
-  then obtain Z \<alpha> \<beta> where \<alpha>1_def: "\<alpha>\<^sub>1 = Z#\<alpha>" and \<alpha>2_def: "\<alpha>\<^sub>2 = \<beta> @ \<alpha>" and trans: "(p\<^sub>2, \<beta>) \<in> trans_fun M p\<^sub>1 End_marker Z"
-    using step\<^sub>1_rule_ext by auto
-  from trans have "(P p\<^sub>2, \<beta>) \<in> trans_fun end_check_dpda (N p\<^sub>1) End_marker Z"
-    using end_check_dpda_trans_marker_N by simp
-  with \<alpha>1_def \<alpha>2_def show ?r
-    using pda.step\<^sub>1_rule[OF pda_end_check] by simp
-next 
-  assume ?r
-  then obtain Z \<alpha> \<beta> where \<alpha>1_def: "\<alpha>\<^sub>1 = Z#\<alpha>" and \<alpha>2_def: "\<alpha>\<^sub>2 = \<beta> @ \<alpha>" and trans: "(P p\<^sub>2, \<beta>) \<in> trans_fun end_check_dpda (N p\<^sub>1) End_marker Z"
-    using pda.step\<^sub>1_rule_ext[OF pda_end_check] by auto
-  from trans have "(p\<^sub>2, \<beta>) \<in> trans_fun M p\<^sub>1 End_marker Z"
-    using end_check_dpda_trans_marker_N by simp
-  with \<alpha>1_def \<alpha>2_def show ?l
-    using step\<^sub>1_rule by simp
-qed
+    pda.step\<^sub>1 end_check_dpda (N p\<^sub>1, End_marker#w, \<alpha>\<^sub>1) (P p\<^sub>2, w, \<alpha>\<^sub>2)"
+by (use step\<^sub>1_rule_ext end_check_dpda_def pda.step\<^sub>1_rule_ext[OF pda_end_check] in auto)
+
+lemma end_check_dpda_P_step\<^sub>1:
+  "pda.step\<^sub>1 M (p\<^sub>1, w\<^sub>1, \<alpha>\<^sub>1) (p\<^sub>2, w\<^sub>2, \<alpha>\<^sub>2) \<longleftrightarrow>
+    pda.step\<^sub>1 end_check_dpda (P p\<^sub>1, w\<^sub>1, \<alpha>\<^sub>1) (P p\<^sub>2, w\<^sub>2, \<alpha>\<^sub>2)"
+by (use step\<^sub>1_rule_ext end_check_dpda_def pda.step\<^sub>1_rule_ext[OF pda_end_check] in auto)
 
 lemma end_check_dpda_input_in_N:
   assumes "pda.step\<^sub>1 end_check_dpda (N p, map Input w\<^sub>1, \<alpha>\<^sub>1) (q, w\<^sub>2, \<alpha>\<^sub>2)"
   shows "\<exists>q'. q = N q'"
-proof -
-  from assms obtain Z \<alpha> where
-  "(\<exists>\<beta>. w\<^sub>2 = map Input w\<^sub>1 \<and> \<alpha>\<^sub>2 = \<beta> @ \<alpha> \<and> (q, \<beta>) \<in> end_check_eps_fun (N p) Z) \<or>
-    (\<exists>a \<beta>. map Input w\<^sub>1 = Input a # w\<^sub>2 \<and> \<alpha>\<^sub>2 = \<beta> @ \<alpha> \<and> (q, \<beta>) \<in> end_check_trans_fun (N p) (Input a) Z)"
-    using pda.step\<^sub>1_rule_ext[OF pda_end_check] by (fastforce simp: end_check_dpda_def)
-  thus ?thesis
-    by (induction "N p" Z rule: end_check_eps_fun.induct) auto
-qed
+by (use assms end_check_dpda_def pda.step\<^sub>1_rule_ext[OF pda_end_check] in auto)
+
+lemma end_check_dpda_marker_in_N:
+  assumes "pda.step\<^sub>1 end_check_dpda (N p, End_marker#w, \<alpha>\<^sub>1) (q, w, \<alpha>\<^sub>2)"
+  shows "\<exists>q'. q = P q'"
+by (use assms end_check_dpda_def pda.step\<^sub>1_rule_ext[OF pda_end_check] in auto)
 
 lemma end_check_dpda_inputs_in_N:
   assumes "pda.steps end_check_dpda (N p, map Input w\<^sub>1, \<alpha>\<^sub>1) (q, w\<^sub>2, \<alpha>\<^sub>2)"
   shows "\<exists>q'. q = N q'"
-using assms proof (induction "(N p, map Input w\<^sub>1, \<alpha>\<^sub>1)" "(q, w\<^sub>2, \<alpha>\<^sub>2)" arbitrary: p w\<^sub>1 \<alpha>\<^sub>1 rule: pda.steps_induct[OF pda_end_check])
-  case (3 \<alpha>\<^sub>1 p' w' \<alpha>')
-  from 3(1) obtain p'' where p'_def: "p' = N p''"
-    using end_check_dpda_input_in_N by blast
-  from 3(1) obtain w'' where w'_def: "w' = map Input w''"
-    using pda.step\<^sub>1_rule_ext[OF pda_end_check] by blast
-  from p'_def w'_def 3(2,3) show ?case by simp
-qed (auto simp: assms)
+  by (induction "(N p, map Input w\<^sub>1, \<alpha>\<^sub>1)" "(q, w\<^sub>2, \<alpha>\<^sub>2)" arbitrary: p w\<^sub>1 \<alpha>\<^sub>1 rule: pda.steps_induct[OF pda_end_check])
+       (use assms end_check_dpda_input_in_N pda.step\<^sub>1_rule_ext[OF pda_end_check] in blast)+
 
-lemma end_check_dpda_inputs_from_P:
-  assumes "pda.steps end_check_dpda (p, map Input w\<^sub>1, \<alpha>\<^sub>1) (P q, w\<^sub>2, \<alpha>\<^sub>2)"
-  shows "\<exists>p'. p = P p'"
-proof (rule ccontr)
-  assume "\<nexists>p'. p = P p'"
-  then obtain p' where "p = N p'"
-    using st_primed.exhaust[of p] by auto
-  with assms show False
-    using end_check_dpda_inputs_in_N by blast
-qed
-
-lemma end_check_dpda_input_stepn:
+lemma end_check_dpda_input_in_N_stepn:
   "pda.stepn M n (p\<^sub>1, map Input w, \<alpha>\<^sub>1) (p\<^sub>2, [], \<alpha>\<^sub>2) \<longleftrightarrow>
     pda.stepn end_check_dpda n (N p\<^sub>1, map Input w, \<alpha>\<^sub>1) (N p\<^sub>2, [], \<alpha>\<^sub>2)" (is "?l \<longleftrightarrow> ?r")
 proof 
@@ -262,7 +142,7 @@ proof
       using pda.stepn_split_first[OF pda_end_check] by blast
   qed (simp add: pda.refl\<^sub>n[OF pda_end_check])
 next
-  assume asm: ?r
+  assume r: ?r
   thus ?l proof (induction n "(N p\<^sub>1, map Input w, \<alpha>\<^sub>1)" "(N p\<^sub>2, [] :: 'a input_with_marker list, \<alpha>\<^sub>2)" 
                             arbitrary: p\<^sub>1 w \<alpha>\<^sub>1 rule: pda.stepn_induct[OF pda_end_check])
     case (3 n \<alpha>\<^sub>1 p' w' \<alpha>')
@@ -278,90 +158,15 @@ next
 
     ultimately show ?case
       using stepn_split_first by blast
-  qed (simp_all add: asm)
-qed
-
-lemma end_check_dpda_P_step\<^sub>1:
-  "pda.step\<^sub>1 M (p\<^sub>1, w\<^sub>1, \<alpha>\<^sub>1) (p\<^sub>2, w\<^sub>2, \<alpha>\<^sub>2) \<longleftrightarrow>
-    pda.step\<^sub>1 end_check_dpda (P p\<^sub>1, w\<^sub>1, \<alpha>\<^sub>1) (P p\<^sub>2, w\<^sub>2, \<alpha>\<^sub>2)" (is "?l \<longleftrightarrow> ?r")
-proof
-  assume ?l
-  then obtain Z \<alpha> where \<alpha>1_def: "\<alpha>\<^sub>1 = Z#\<alpha>" and rule: 
-        "(\<exists>\<beta>. w\<^sub>2 = w\<^sub>1 \<and> \<alpha>\<^sub>2 = \<beta> @ \<alpha> \<and> (p\<^sub>2, \<beta>) \<in> eps_fun M p\<^sub>1 Z) \<or>
-            (\<exists>a \<beta>. w\<^sub>1 = a # w\<^sub>2 \<and> \<alpha>\<^sub>2 = \<beta> @ \<alpha> \<and> (p\<^sub>2, \<beta>) \<in> trans_fun M p\<^sub>1 a Z)"
-    using step\<^sub>1_rule_ext by auto
-  from rule have "(\<exists>\<beta>. w\<^sub>2 = w\<^sub>1 \<and> \<alpha>\<^sub>2 = \<beta> @ \<alpha> \<and> (P p\<^sub>2, \<beta>) \<in> eps_fun end_check_dpda (P p\<^sub>1) Z) \<or>
-            (\<exists>a \<beta>. w\<^sub>1 = a # w\<^sub>2 \<and> \<alpha>\<^sub>2 = \<beta> @ \<alpha> \<and> (P p\<^sub>2, \<beta>) \<in> trans_fun end_check_dpda (P p\<^sub>1) a Z)"
-    using end_check_dpda_eps_P end_check_dpda_trans_P by simp
-  with \<alpha>1_def show ?r
-    using pda.step\<^sub>1_rule[OF pda_end_check] by simp
-next
-  assume ?r
-  then obtain Z \<alpha> where \<alpha>1_def: "\<alpha>\<^sub>1 = Z#\<alpha>" and rule: 
-        "(\<exists>\<beta>. w\<^sub>2 = w\<^sub>1 \<and> \<alpha>\<^sub>2 = \<beta> @ \<alpha> \<and> (P p\<^sub>2, \<beta>) \<in> eps_fun end_check_dpda (P p\<^sub>1) Z) \<or>
-            (\<exists>a \<beta>. w\<^sub>1 = a # w\<^sub>2 \<and> \<alpha>\<^sub>2 = \<beta> @ \<alpha> \<and> (P p\<^sub>2, \<beta>) \<in> trans_fun end_check_dpda (P p\<^sub>1) a Z)"
-    using pda.step\<^sub>1_rule_ext[OF pda_end_check] by auto
-  from rule have "(\<exists>\<beta>. w\<^sub>2 = w\<^sub>1 \<and> \<alpha>\<^sub>2 = \<beta> @ \<alpha> \<and> (p\<^sub>2, \<beta>) \<in> eps_fun M p\<^sub>1 Z) \<or>
-            (\<exists>a \<beta>. w\<^sub>1 = a # w\<^sub>2 \<and> \<alpha>\<^sub>2 = \<beta> @ \<alpha> \<and> (p\<^sub>2, \<beta>) \<in> trans_fun M p\<^sub>1 a Z)"
-    using end_check_dpda_eps_P end_check_dpda_trans_P by simp
-  with \<alpha>1_def show ?l
-    using step\<^sub>1_rule by simp
-qed
+  qed (rule r, simp)
+qed 
 
 lemma end_check_dpda_in_P:
   assumes "pda.step\<^sub>1 end_check_dpda (P p, w\<^sub>1, \<alpha>\<^sub>1) (q, w\<^sub>2, \<alpha>\<^sub>2)"
   shows "\<exists>q'. q = P q'"
-proof - 
-  thm pda.step\<^sub>1_rule[OF pda_end_check]
-  from assms obtain Z \<alpha> where 
-    "(\<exists>\<beta>. w\<^sub>2 = w\<^sub>1 \<and> \<alpha>\<^sub>2 = \<beta> @ \<alpha> \<and> (q, \<beta>) \<in> end_check_eps_fun (P p) Z) \<or>
-      (\<exists>a \<beta>. w\<^sub>1 = a # w\<^sub>2 \<and> \<alpha>\<^sub>2 = \<beta> @ \<alpha> \<and> (q, \<beta>) \<in> end_check_trans_fun (P p) a Z)"
-    using pda.step\<^sub>1_rule_ext[OF pda_end_check] by (fastforce simp: end_check_dpda_def)
-  thus ?thesis
-    by (induction "P p" Z rule: end_check_eps_fun.induct) auto
-qed
+by (use assms end_check_dpda_def pda.step\<^sub>1_rule_ext[OF pda_end_check] in auto)
 
-lemma end_check_dpda_ins_P:
-  assumes "pda.steps end_check_dpda (P p, w\<^sub>1, \<alpha>\<^sub>1) (q, w\<^sub>2, \<alpha>\<^sub>2)"
-  shows "\<exists>q'. q = P q'"
-using assms by (induction "(P p, w\<^sub>1, \<alpha>\<^sub>1)" "(q, w\<^sub>2, \<alpha>\<^sub>2)" arbitrary: p w\<^sub>1 \<alpha>\<^sub>1 rule: pda.steps_induct[OF pda_end_check])
-                  (blast intro: assms dest: end_check_dpda_in_P)+
-
-lemma end_check_dpda_marker_in_N:
-  assumes "pda.step\<^sub>1 end_check_dpda (N p, [End_marker], \<alpha>\<^sub>1) (q, [], \<alpha>\<^sub>2)"
-  shows "\<exists>q'. q = P q'"
-proof -
-  from assms obtain Z \<beta> where "(q, \<beta>) \<in> end_check_trans_fun (N p) End_marker Z"
-    using pda.step\<^sub>1_rule_ext[OF pda_end_check] by (fastforce simp: end_check_dpda_def)
-  thus ?thesis
-    by (induction "N p" "End_marker :: 'a input_with_marker" Z rule: end_check_trans_fun.induct) auto
-qed
-
-lemma end_check_dpda_marker_ins_N:
-  assumes "pda.steps end_check_dpda (N p, [End_marker], \<alpha>\<^sub>1) (q, [], \<alpha>\<^sub>2)"
-  shows "\<exists>q'. q = P q'"
-proof -
-  thm pda.stepn_reads_input[OF pda_end_check]
-  from assms obtain n where stepn: "pda.stepn end_check_dpda n (N p, [End_marker], \<alpha>\<^sub>1) (q, [], \<alpha>\<^sub>2)"
-    using pda.stepn_steps[OF pda_end_check] by blast
-  then obtain n' where "n = Suc n'"
-    using pda.stepn_not_refl_split_first[OF pda_end_check] by blast
-  with stepn obtain q\<^sub>1 q\<^sub>2 \<gamma>\<^sub>1 \<gamma>\<^sub>2 where 
-          toq1: "pda.steps end_check_dpda (N p, [End_marker], \<alpha>\<^sub>1) (q\<^sub>1, [End_marker], \<gamma>\<^sub>1)" and
-          toq2: "pda.step\<^sub>1 end_check_dpda (q\<^sub>1, [End_marker], \<gamma>\<^sub>1) (q\<^sub>2, [], \<gamma>\<^sub>2)" and 
-          toq: "pda.steps end_check_dpda (q\<^sub>2, [], \<gamma>\<^sub>2) (q, [], \<alpha>\<^sub>2)"
-    using pda.stepn_reads_input[OF pda_end_check] pda.stepn_steps[OF pda_end_check] by metis
-  from toq1 have "pda.steps end_check_dpda (N p, [], \<alpha>\<^sub>1) (q\<^sub>1, [], \<gamma>\<^sub>1)"
-    using pda.steps_word_app[OF pda_end_check] by fastforce
-  then obtain q\<^sub>1' where "q\<^sub>1 = N q\<^sub>1'"
-    using end_check_dpda_inputs_in_N[of p "[]" \<alpha>\<^sub>1 q\<^sub>1 "[]" \<gamma>\<^sub>1] by auto
-  with toq2 obtain q\<^sub>2' where "q\<^sub>2 = P q\<^sub>2'"
-    using end_check_dpda_marker_in_N by blast
-  with toq show ?thesis
-    using end_check_dpda_ins_P by simp
-qed
-
-lemma end_check_dpda_P_stepn:
+lemma end_check_dpda_in_P_stepn:
   "pda.stepn M n (p\<^sub>1, w\<^sub>1, \<alpha>\<^sub>1) (p\<^sub>2, w\<^sub>2, \<alpha>\<^sub>2) \<longleftrightarrow>
     pda.stepn end_check_dpda n (P p\<^sub>1, w\<^sub>1, \<alpha>\<^sub>1) (P p\<^sub>2, w\<^sub>2, \<alpha>\<^sub>2)" (is "?l \<longleftrightarrow> ?r")
 proof
@@ -374,7 +179,7 @@ proof
       using pda.step\<^sub>n[OF pda_end_check] by simp
   qed (simp add: pda.refl\<^sub>n[OF pda_end_check])
 next
-  assume asm: ?r
+  assume r: ?r
   thus ?l
   proof (induction n "(P p\<^sub>1, w\<^sub>1, \<alpha>\<^sub>1)" "(P p\<^sub>2, w\<^sub>2, \<alpha>\<^sub>2)" arbitrary: p\<^sub>1 w\<^sub>1 \<alpha>\<^sub>1 rule: pda.stepn_induct[OF pda_end_check])
     case (3 n w\<^sub>1 \<alpha>\<^sub>1 p' w' \<alpha>')
@@ -388,7 +193,7 @@ next
 
     ultimately show ?case
       using stepn_split_first by blast
-  qed (simp_all add: asm)
+  qed (rule r, simp)
 qed
 
 lemma end_check_dpda_marker_stepn:
@@ -396,50 +201,50 @@ lemma end_check_dpda_marker_stepn:
     pda.stepn end_check_dpda n (N p\<^sub>1, [End_marker], \<alpha>\<^sub>1) (P p\<^sub>2, [], \<alpha>\<^sub>2)" (is "?l \<longleftrightarrow> ?r")
 proof
   assume l: ?l
-  then obtain n' where n_def: "n = Suc n'"
-    using stepn_not_refl gr0_implies_Suc by blast
-  with l obtain k q\<^sub>1 q\<^sub>2 \<gamma>\<^sub>1 \<gamma>\<^sub>2 where k_less: "k \<le> n'" and stepk: "stepn k (p\<^sub>1, [End_marker], \<alpha>\<^sub>1) (q\<^sub>1, [End_marker], \<gamma>\<^sub>1)"
+  obtain n' k q\<^sub>1 q\<^sub>2 \<gamma>\<^sub>1 \<gamma>\<^sub>2 where n_def: "n = Suc n'" and k_less: "k \<le> n'" and stepk: "stepn k (p\<^sub>1, [End_marker], \<alpha>\<^sub>1) (q\<^sub>1, [End_marker], \<gamma>\<^sub>1)"
     and step1: "step\<^sub>1 (q\<^sub>1, [End_marker], \<gamma>\<^sub>1) (q\<^sub>2, [], \<gamma>\<^sub>2)" and stepn'k: "stepn (n' - k) (q\<^sub>2, [], \<gamma>\<^sub>2) (p\<^sub>2, [], \<alpha>\<^sub>2)"
-    using stepn_reads_input[of n' p\<^sub>1 End_marker "[]" \<alpha>\<^sub>1 p\<^sub>2 \<alpha>\<^sub>2] by auto
+    using stepn_reads_input[OF l] by blast 
   from stepk have "stepn k (p\<^sub>1, [], \<alpha>\<^sub>1) (q\<^sub>1, [], \<gamma>\<^sub>1)"
     using stepn_word_app[of k p\<^sub>1 "[]" \<alpha>\<^sub>1 q\<^sub>1 "[]" \<gamma>\<^sub>1 "[End_marker]"] by simp
   hence "pda.stepn end_check_dpda k (N p\<^sub>1, [], \<alpha>\<^sub>1) (N q\<^sub>1, [], \<gamma>\<^sub>1)"
-    using end_check_dpda_input_stepn[where ?w = "[]"] by simp
+    using end_check_dpda_input_in_N_stepn[where ?w = "[]"] by simp
 
-  hence "pda.stepn end_check_dpda k (N p\<^sub>1, [End_marker], \<alpha>\<^sub>1) (N q\<^sub>1, [End_marker], \<gamma>\<^sub>1)"
+  hence *: "pda.stepn end_check_dpda k (N p\<^sub>1, [End_marker], \<alpha>\<^sub>1) (N q\<^sub>1, [End_marker], \<gamma>\<^sub>1)"
     using pda.stepn_word_app[OF pda_end_check, of k "N p\<^sub>1" "[]" \<alpha>\<^sub>1 "N q\<^sub>1" "[]" \<gamma>\<^sub>1 "[End_marker]"] by simp
 
-  moreover from step1 have "pda.step\<^sub>1 end_check_dpda (N q\<^sub>1, [End_marker], \<gamma>\<^sub>1) (P q\<^sub>2, [], \<gamma>\<^sub>2)"
+  from step1 have **: "pda.step\<^sub>1 end_check_dpda (N q\<^sub>1, [End_marker], \<gamma>\<^sub>1) (P q\<^sub>2, [], \<gamma>\<^sub>2)"
     using end_check_dpda_marker_step\<^sub>1 by simp
 
-  moreover from stepn'k have "pda.stepn end_check_dpda (n' - k) (P q\<^sub>2, [], \<gamma>\<^sub>2) (P p\<^sub>2, [], \<alpha>\<^sub>2)" 
-    using end_check_dpda_P_stepn by simp
+  from stepn'k have ***: "pda.stepn end_check_dpda (n' - k) (P q\<^sub>2, [], \<gamma>\<^sub>2) (P p\<^sub>2, [], \<alpha>\<^sub>2)" 
+    using end_check_dpda_in_P_stepn by simp
 
-  ultimately show ?r 
-    using n_def k_less pda.step\<^sub>n[OF pda_end_check] pda.stepn_trans[OF pda_end_check] by fastforce
+  from n_def k_less show ?r 
+    using pda.stepn_trans[OF pda_end_check pda.step\<^sub>n[OF pda_end_check * **] ***] by simp
 next
   assume r: ?r
-  then obtain n' where n_def: "n = Suc n'"
-    using pda.stepn_not_refl[OF pda_end_check] gr0_implies_Suc by blast
-  with r obtain k q\<^sub>1 q\<^sub>2 \<gamma>\<^sub>1 \<gamma>\<^sub>2 where k_less: "k \<le> n'" and 
+  obtain n' k q\<^sub>1 q\<^sub>2 \<gamma>\<^sub>1 \<gamma>\<^sub>2 where n_def: "n = Suc n'" and k_less: "k \<le> n'" and 
           stepk: "pda.stepn end_check_dpda k (N p\<^sub>1, [End_marker], \<alpha>\<^sub>1) (q\<^sub>1, [End_marker], \<gamma>\<^sub>1)" and
           step1: "pda.step\<^sub>1 end_check_dpda (q\<^sub>1, [End_marker], \<gamma>\<^sub>1) (q\<^sub>2, [], \<gamma>\<^sub>2)" and
           stepn'k: "pda.stepn end_check_dpda (n' - k) (q\<^sub>2, [], \<gamma>\<^sub>2) (P p\<^sub>2, [], \<alpha>\<^sub>2)"
-    using pda.stepn_reads_input[OF pda_end_check] by blast
+    using pda.stepn_reads_input[OF pda_end_check r] by blast
   from stepk have stepk_emp: "pda.stepn end_check_dpda k (N p\<^sub>1, [], \<alpha>\<^sub>1) (q\<^sub>1, [], \<gamma>\<^sub>1)"
     using pda.stepn_word_app[OF pda_end_check] by fastforce
   then obtain q\<^sub>1' where q1_def: "q\<^sub>1 = N q\<^sub>1'"
     using pda.stepn_steps[OF pda_end_check] end_check_dpda_inputs_in_N[of p\<^sub>1 "[]" \<alpha>\<^sub>1 q\<^sub>1 "[]" \<gamma>\<^sub>1] by fastforce
   with stepk_emp have "stepn k (p\<^sub>1, [], \<alpha>\<^sub>1) (q\<^sub>1', [], \<gamma>\<^sub>1)"
-    using end_check_dpda_input_stepn[where ?w = "[]"] by simp
+    using end_check_dpda_input_in_N_stepn[where ?w = "[]"] by simp
+
   hence *: "stepn k (p\<^sub>1, [End_marker], \<alpha>\<^sub>1) (q\<^sub>1', [End_marker], \<gamma>\<^sub>1)"
     using stepn_word_app[of k p\<^sub>1 "[]" \<alpha>\<^sub>1 q\<^sub>1' "[]" \<gamma>\<^sub>1 "[End_marker]"] by simp
-  from stepn'k obtain q\<^sub>2' where q2_def: "q\<^sub>2 = P q\<^sub>2'"
-    using pda.stepn_steps[OF pda_end_check] end_check_dpda_inputs_from_P[of q\<^sub>2 "[]" \<gamma>\<^sub>2 p\<^sub>2 "[]" \<alpha>\<^sub>2] by fastforce
+  from step1 q1_def obtain q\<^sub>2' where q2_def: "q\<^sub>2 = P q\<^sub>2'"
+    using end_check_dpda_marker_in_N by blast
+
   with stepn'k have **: "stepn (n' - k) (q\<^sub>2', [], \<gamma>\<^sub>2) (p\<^sub>2, [], \<alpha>\<^sub>2)"
-    using end_check_dpda_P_stepn by simp
+    using end_check_dpda_in_P_stepn by simp
+
   from q1_def q2_def step1 have ***: "step\<^sub>1 (q\<^sub>1', [End_marker], \<gamma>\<^sub>1) (q\<^sub>2', [], \<gamma>\<^sub>2)"
     using end_check_dpda_marker_step\<^sub>1 by simp
+
   from n_def k_less show ?l 
     using stepn_trans[OF step\<^sub>n[OF * ***] **] by simp
 qed
@@ -448,30 +253,30 @@ lemma end_check_dpda_stepn:
   "pda.stepn M n (p\<^sub>1, word_with_end w, \<alpha>\<^sub>1) (p\<^sub>2, [], \<alpha>\<^sub>2) \<longleftrightarrow>
      pda.stepn end_check_dpda n (N p\<^sub>1, word_with_end w, \<alpha>\<^sub>1) (P p\<^sub>2, [], \<alpha>\<^sub>2)" (is "?l \<longleftrightarrow> ?r")
 proof
-  assume ?l
-  then obtain k q \<gamma> where k_less: "k \<le> n" and stepk: "pda.stepn M k (p\<^sub>1, map Input w, \<alpha>\<^sub>1) (q, [], \<gamma>)" 
-                            and stepnk: "pda.stepn M (n-k) (q, [End_marker], \<gamma>) (p\<^sub>2, [], \<alpha>\<^sub>2)"
-    using split_word by blast
+  assume l: ?l
+  obtain k q \<gamma> where k_less: "k \<le> n" and stepk: "pda.stepn M k (p\<^sub>1, map Input w, \<alpha>\<^sub>1) (q, [], \<gamma>)" 
+                            and stepnk: "pda.stepn M (n - k) (q, [End_marker], \<gamma>) (p\<^sub>2, [], \<alpha>\<^sub>2)"
+    using split_word[OF l] by blast
   from stepk have "pda.stepn end_check_dpda k (N p\<^sub>1, map Input w, \<alpha>\<^sub>1) (N q, [], \<gamma>)"
-    using end_check_dpda_input_stepn by simp
+    using end_check_dpda_input_in_N_stepn by simp
 
   hence "pda.stepn end_check_dpda k (N p\<^sub>1, word_with_end w, \<alpha>\<^sub>1) (N q, [End_marker], \<gamma>)"
     using pda.stepn_word_app[OF pda_end_check, of k "N p\<^sub>1" "map Input w" "\<alpha>\<^sub>1" "N q" "[]" \<gamma> "[End_marker]"] by simp 
 
-  moreover from stepnk have "pda.stepn end_check_dpda (n-k) (N q, [End_marker], \<gamma>) (P p\<^sub>2, [], \<alpha>\<^sub>2)"
+  moreover from stepnk have "pda.stepn end_check_dpda (n - k) (N q, [End_marker], \<gamma>) (P p\<^sub>2, [], \<alpha>\<^sub>2)"
     using end_check_dpda_marker_stepn by simp
 
   ultimately show ?r
     using k_less pda.stepn_trans[OF pda_end_check] by fastforce 
 next
-  assume ?r
-  then obtain k q \<gamma> where k_less: "k \<le> n" and stepk: "pda.stepn end_check_dpda k (N p\<^sub>1, map Input w, \<alpha>\<^sub>1) (q, [], \<gamma>)"
-                      and stepnk: "pda.stepn end_check_dpda (n-k) (q, [End_marker], \<gamma>) (P p\<^sub>2, [], \<alpha>\<^sub>2)"
-    using pda.split_word[OF pda_end_check] by blast
+  assume r: ?r
+  obtain k q \<gamma> where k_less: "k \<le> n" and stepk: "pda.stepn end_check_dpda k (N p\<^sub>1, map Input w, \<alpha>\<^sub>1) (q, [], \<gamma>)"
+                      and stepnk: "pda.stepn end_check_dpda (n - k) (q, [End_marker], \<gamma>) (P p\<^sub>2, [], \<alpha>\<^sub>2)"
+    using pda.split_word[OF pda_end_check r] by blast
   from stepk obtain q' where q_def: "q = N q'" 
     using pda.stepn_steps[OF pda_end_check] end_check_dpda_inputs_in_N by blast
   with stepk have "pda.stepn M k (p\<^sub>1, map Input w, \<alpha>\<^sub>1) (q', [], \<gamma>)"
-    using end_check_dpda_input_stepn by simp
+    using end_check_dpda_input_in_N_stepn by simp
 
   hence "pda.stepn M k (p\<^sub>1, word_with_end w, \<alpha>\<^sub>1) (q', [End_marker], \<gamma>)"
     using stepn_word_app[of k p\<^sub>1 "map Input w" \<alpha>\<^sub>1 q' "[]" \<gamma> "[End_marker]"] by simp
@@ -490,7 +295,7 @@ lemma accepted_end_check:
   assume ?l
   then obtain q \<gamma> where q_final: "q \<in> final_states M" and steps: "steps (init_state M, word_with_end w, [init_symbol M]) (q, [], \<gamma>)" by blast
   from q_final have *: "P q \<in> final_states end_check_dpda"
-    unfolding end_check_dpda_def end_check_final_states_def by simp
+    by (simp add: end_check_dpda_def end_check_final_states_def)
   from steps have "pda.steps end_check_dpda (N (init_state M), word_with_end w, [init_symbol M]) (P q, [], \<gamma>)"
     using stepn_steps end_check_dpda_stepn[where ?w = w and ?\<alpha>\<^sub>1 = "[init_symbol M]" and ?\<alpha>\<^sub>2 = \<gamma>] 
            pda.stepn_steps[OF pda_end_check] by blast
@@ -514,25 +319,7 @@ qed
 
 lemma lang_end_check_dpda:
   "dpda.final_accept_det M = dpda.final_accept_det end_check_dpda"
-unfolding final_accept_det_def dpda.final_accept_det_def[OF dpda_end_check] using accepted_end_check by blast
-
-lemma finished_end_check_dpda:
-  assumes "pda.steps end_check_dpda (p, word_with_end w\<^sub>1, \<alpha>\<^sub>1) (q, [], \<alpha>\<^sub>2)"
-  shows "\<exists>q'. q = P q'"
-proof (cases p)
-  case (N p')
-  with assms obtain q' \<gamma>' where toq': "pda.steps end_check_dpda (N p', map Input w\<^sub>1, \<alpha>\<^sub>1) (q', [], \<gamma>')" and
-                                  toq: "pda.steps end_check_dpda (q', [End_marker], \<gamma>') (q, [], \<alpha>\<^sub>2)"
-    using pda.stepn_steps[OF pda_end_check] pda.split_word[OF pda_end_check] by metis
-  from toq' obtain q'' where "q' = N q''"
-    using end_check_dpda_inputs_in_N by blast
-  with toq show ?thesis
-    using end_check_dpda_marker_ins_N by simp
-next
-  case (P p')
-  with assms show ?thesis
-    using end_check_dpda_ins_P by simp
-qed
+unfolding final_accept_det_def dpda.final_accept_det_def[OF dpda_end_check] using accepted_end_check by simp
 
 end
 end
