TaskinBA/DPDA.thy
@@ -27,43 +27,54 @@ next
 qed
 
 locale dpda = pda M for M :: "('q :: finite, ('a :: finite) input_with_marker, 's :: finite) pda" +
-  assumes det: "card (trans_fun M q a Z) + card (eps_fun M q Z) \<le> 1"
+  assumes det: "card (trans_fun M q a Z) + card (eps_fun M q Z) = 1"
       and init_trans: "(q, \<alpha>) \<in> trans_fun M p a (init_symbol M) \<Longrightarrow> \<exists>\<alpha>'. \<alpha> = \<alpha>' @ [init_symbol M]"
       and init_eps: "(q, \<alpha>) \<in> eps_fun M p (init_symbol M) \<Longrightarrow> \<exists>\<alpha>'. \<alpha> = \<alpha>' @ [init_symbol M]"
 begin
 
-(* show that every pda with the assumption det has a dpda accepting the same set and vice versa *)
+(* TODO: show that every pda with the assumption det has a dpda accepting the same set and vice versa *)
 
-lemma step_empty_or_singleton: "step (p, w, Z#\<alpha>) = {} \<or> (\<exists>p' w' \<alpha>'. step (p, w, Z#\<alpha>) = {(p', w', \<alpha>')})"
-proof (cases w)
-  case Nil
-  hence "card (step (p, w, Z # \<alpha>)) = card (eps_fun M p Z)"
+lemma dpda_step_empty_word: "step (p, [], Z#\<alpha>) = {} \<or> (\<exists>p' w' \<alpha>'. step (p, [], Z#\<alpha>) = {(p', w', \<alpha>')})"
+proof -
+  have "card (step (p, [], Z#\<alpha>)) = card (eps_fun M p Z)"
     using card_empty_step by simp
   also have "... \<le> 1"
     using det[where ?q = p and ?Z = Z] by fastforce
   finally show ?thesis
-    using card_leq_1[OF finite_step] by simp
-next
-  case (Cons a w')
-  hence "card (step (p, w, Z#\<alpha>)) = card (trans_fun M p a Z) + card (eps_fun M p Z)"
-    using card_nonempty_step by simp
-  also have "... \<le> 1"
-    using det by simp
-  finally show ?thesis
-    using card_leq_1[OF finite_step] by simp
+    using card_leq_1[OF finite_step[of _ "[]"]] by simp
 qed
 
-lemma step_det:
+lemma dpda_step_nonempty_word: "\<exists>p' w' \<alpha>'. step (p, a#w, Z#\<alpha>) = {(p', w', \<alpha>')}"
+proof -
+  have "card (step (p, a#w, Z#\<alpha>)) = card (trans_fun M p a Z) + card (eps_fun M p Z)"
+    using card_nonempty_step by simp
+  also have "... = 1"
+    using det by simp
+  finally show ?thesis
+    by (simp add: card_1_singleton_iff)
+qed
+
+lemma dpda_step_det:
   assumes "step\<^sub>1 (p, w, \<alpha>) (q, y, \<gamma>)"
       and "step\<^sub>1 (p, w, \<alpha>) (q', y', \<gamma>')"
     shows "q = q' \<and> y = y' \<and> \<gamma> = \<gamma>'"
-using assms step\<^sub>1_nonempty_stack[of p w \<alpha> q y \<gamma>] step_empty_or_singleton[of p w] by force 
+proof (cases w)
+  case Nil
+  with assms(1) have "step (p, w, \<alpha>) = {} \<or> (\<exists>p' w' \<alpha>'. step (p, w, \<alpha>) = {(p', w', \<alpha>')})"
+    using step\<^sub>1_nonempty_stack[of p w \<alpha> q y \<gamma>] dpda_step_empty_word[of p] by blast
+  with assms show ?thesis by auto
+next
+  case (Cons a w')
+  with assms(1) have "\<exists>p' w' \<alpha>'. step (p, w, \<alpha>) = {(p', w', \<alpha>')}"
+    using step\<^sub>1_nonempty_stack[of p w \<alpha> q y \<gamma>] dpda_step_nonempty_word by blast
+  with assms show ?thesis by auto
+qed
 
 lemma stepn_det:
   assumes "stepn n (p, w, \<alpha>) (q, y, \<gamma>)"
       and "stepn n (p, w, \<alpha>) (q', y', \<gamma>')"
     shows "q = q' \<and> y = y' \<and> \<gamma> = \<gamma>'"
-using assms by (induction n "(p, w, \<alpha>)" "(q, y, \<gamma>)" arbitrary: q y \<gamma> q' y' \<gamma>' rule: stepn.induct) (fastforce simp: step_det)+
+using assms by (induction n "(p, w, \<alpha>)" "(q, y, \<gamma>)" arbitrary: q y \<gamma> q' y' \<gamma>' rule: stepn.induct) (fastforce simp: dpda_step_det)+
 
 lemma step\<^sub>1_init_bottom:
   assumes "step\<^sub>1 (p\<^sub>1, w\<^sub>1, \<alpha>\<^sub>1 @ [init_symbol M]) (p\<^sub>2, w\<^sub>2, \<alpha>\<^sub>2)"
@@ -76,9 +87,11 @@ lemma steps_init_bottom:
 using assms by (induction "(p\<^sub>1, w\<^sub>1, \<alpha>\<^sub>1 @ [init_symbol M])" " (p\<^sub>2, w\<^sub>2, \<alpha>\<^sub>2)" arbitrary: p\<^sub>1 w\<^sub>1 \<alpha>\<^sub>1 rule: steps_induct) 
                  (fastforce simp: step\<^sub>1_init_bottom)+
 
-abbreviation "word_with_end w \<equiv> map Input w @ [End_marker]"
+abbreviation word_with_end :: "'a list \<Rightarrow> 'a input_with_marker list" where 
+  "word_with_end w \<equiv> map Input w @ [End_marker]"
 
-definition "final_accept_det \<equiv> {w | w q \<gamma>. q \<in> final_states M \<and> steps (init_state M, word_with_end w, [init_symbol M]) (q, [], \<gamma>)}"
+definition final_accept_det :: "'a list set" where
+  "final_accept_det \<equiv> {w | w q \<gamma>. q \<in> final_states M \<and> steps (init_state M, word_with_end w, [init_symbol M]) (q, [], \<gamma>)}"
 
 end
 end
