TaskinBA/Final_To_Stack_PDA.thy
@@ -46,104 +46,86 @@ proof (standard, goal_cases)
   have "finite (final_to_stack_trans_fun p x z)"
     by (induction p x z rule: final_to_stack_trans_fun.induct) (auto simp: finite_trans)
   then show ?case
-    unfolding final_to_stack_pda_def by simp
+    by (simp add: final_to_stack_pda_def)
 next
   case (2 p z)
   have "finite (final_to_stack_eps_fun p z)"
     by (induction p z rule: final_to_stack_eps_fun.induct) (auto simp: finite_eps)
   then show ?case
-    unfolding final_to_stack_pda_def by simp
+    by (simp add: final_to_stack_pda_def)
 qed
 
 lemma final_to_stack_pda_trans:
   "(p, \<beta>) \<in> trans_fun M q a Z \<longleftrightarrow> 
           (Old_st p, map Old_sym \<beta>) \<in> trans_fun final_to_stack_pda (Old_st q) a (Old_sym Z)"
-proof
-  assume "(p, \<beta>) \<in> trans_fun M q a Z"
-  thus "(Old_st p, map Old_sym \<beta>) \<in> trans_fun final_to_stack_pda (Old_st q) a (Old_sym Z)"
-    unfolding final_to_stack_pda_def by auto
-next
-  assume "(Old_st p, map Old_sym \<beta>) \<in> trans_fun final_to_stack_pda (Old_st q) a (Old_sym Z)"
-  hence "(Old_st p, map Old_sym \<beta>) \<in> (\<lambda>(p, \<alpha>). (Old_st p, map Old_sym \<alpha>)) ` (trans_fun M q a Z)"
-    unfolding final_to_stack_pda_def by simp
-  then obtain p' \<alpha>' where old_eq: "(Old_st p, map Old_sym \<beta>) = (Old_st p', map Old_sym \<alpha>')" and elem: "(p', \<alpha>') \<in> (trans_fun M q a Z)" by auto
-  from old_eq have p_eq: "p = p'" by simp
-  from old_eq have \<beta>_eq: "\<beta> = \<alpha>'"
-    by (metis list.inj_map_strong prod.inject sym_extended.inject)
-  from p_eq \<beta>_eq elem show "(p, \<beta>) \<in> trans_fun M q a Z" by simp
-qed
+  apply (rule iffI)
+   apply (auto simp: final_to_stack_pda_def)
+  apply (metis list.inj_map_strong sym_extended.inject)
+  done
 
 lemma final_to_stack_pda_eps:
   "(p, \<beta>) \<in> eps_fun M q Z \<longleftrightarrow> (Old_st p, map Old_sym \<beta>) \<in> eps_fun final_to_stack_pda (Old_st q) (Old_sym Z)"
-proof
-  assume "(p, \<beta>) \<in> eps_fun M q Z"
-  thus "(Old_st p, map Old_sym \<beta>) \<in> eps_fun final_to_stack_pda (Old_st q) (Old_sym Z)"
-    unfolding final_to_stack_pda_def by auto
-next
-  assume "(Old_st p, map Old_sym \<beta>) \<in> eps_fun final_to_stack_pda (Old_st q) (Old_sym Z)"
-  hence "(Old_st p, map Old_sym \<beta>) \<in> (\<lambda>(p, \<alpha>). (Old_st p, map Old_sym \<alpha>)) ` (eps_fun M q Z)"
-    unfolding final_to_stack_pda_def by auto (metis empty_iff fst_conv singletonD st_extended.simps(5))
-  then obtain p' \<alpha>' where old_eq: "(Old_st p, map Old_sym \<beta>) = (Old_st p', map Old_sym \<alpha>')" and elem: "(p', \<alpha>') \<in> (eps_fun M q Z)" by auto
-  from old_eq have p_eq: "p = p'" by simp
-  from old_eq have \<beta>_eq: "\<beta> = \<alpha>'"
-    by (metis list.inj_map_strong prod.inject sym_extended.inject)
-  from p_eq \<beta>_eq elem show "(p, \<beta>) \<in> eps_fun M q Z" by simp
-qed
+  apply (rule iffI)
+   apply (auto simp: final_to_stack_pda_def)
+   apply (meson empty_iff prod.inject singletonD st_extended.distinct(3))
+  apply (metis list.inj_map_strong sym_extended.inject)
+  done
 
 lemma final_to_stack_pda_step:
   "pda.step\<^sub>1 M (p\<^sub>1, w\<^sub>1, \<alpha>\<^sub>1) (p\<^sub>2, w\<^sub>2, \<alpha>\<^sub>2) \<longleftrightarrow>
-             pda.step\<^sub>1 final_to_stack_pda (Old_st p\<^sub>1, w\<^sub>1, map Old_sym \<alpha>\<^sub>1) (Old_st p\<^sub>2, w\<^sub>2, map Old_sym \<alpha>\<^sub>2)"
+             pda.step\<^sub>1 final_to_stack_pda (Old_st p\<^sub>1, w\<^sub>1, map Old_sym \<alpha>\<^sub>1) (Old_st p\<^sub>2, w\<^sub>2, map Old_sym \<alpha>\<^sub>2)" (is "?l \<longleftrightarrow> ?r")
 proof
-  assume "pda.step\<^sub>1 M (p\<^sub>1, w\<^sub>1, \<alpha>\<^sub>1) (p\<^sub>2, w\<^sub>2, \<alpha>\<^sub>2)"
-  then obtain Z' \<alpha>' where \<alpha>\<^sub>1_def: "\<alpha>\<^sub>1 = Z'#\<alpha>'" and rule: 
-              "(\<exists>\<beta>. w\<^sub>2 = w\<^sub>1 \<and> \<alpha>\<^sub>2 = \<beta>@\<alpha>' \<and> (p\<^sub>2, \<beta>) \<in> eps_fun M p\<^sub>1 Z') 
-                 \<or> (\<exists>a \<beta>. w\<^sub>1 = a # w\<^sub>2 \<and> \<alpha>\<^sub>2 = \<beta>@\<alpha>' \<and> (p\<^sub>2,\<beta>) \<in> trans_fun M p\<^sub>1 a Z')"
+  assume ?l
+  then obtain Z \<alpha> where \<alpha>\<^sub>1_def: "\<alpha>\<^sub>1 = Z#\<alpha>" and rule: 
+              "(\<exists>\<beta>. w\<^sub>2 = w\<^sub>1 \<and> \<alpha>\<^sub>2 = \<beta>@\<alpha> \<and> (p\<^sub>2, \<beta>) \<in> eps_fun M p\<^sub>1 Z) 
+                 \<or> (\<exists>a \<beta>. w\<^sub>1 = a # w\<^sub>2 \<and> \<alpha>\<^sub>2 = \<beta>@\<alpha> \<and> (p\<^sub>2,\<beta>) \<in> trans_fun M p\<^sub>1 a Z)"
     using step\<^sub>1_rule_ext by auto
-  from rule have "(\<exists>\<beta>. w\<^sub>2 = w\<^sub>1 \<and> map Old_sym \<alpha>\<^sub>2 = map Old_sym \<beta> @ map Old_sym \<alpha>' \<and> 
-                    (Old_st p\<^sub>2, map Old_sym \<beta>) \<in> eps_fun final_to_stack_pda (Old_st p\<^sub>1) (Old_sym Z')) 
-                \<or> (\<exists>a \<beta>. w\<^sub>1 = a # w\<^sub>2 \<and> map Old_sym \<alpha>\<^sub>2 = map Old_sym \<beta> @ map Old_sym \<alpha>' \<and> 
-                    (Old_st p\<^sub>2, map Old_sym \<beta>) \<in> trans_fun final_to_stack_pda (Old_st p\<^sub>1) a (Old_sym Z'))"
+  from rule have "(\<exists>\<beta>. w\<^sub>2 = w\<^sub>1 \<and> map Old_sym \<alpha>\<^sub>2 = map Old_sym \<beta> @ map Old_sym \<alpha> \<and> 
+                    (Old_st p\<^sub>2, map Old_sym \<beta>) \<in> eps_fun final_to_stack_pda (Old_st p\<^sub>1) (Old_sym Z)) 
+                \<or> (\<exists>a \<beta>. w\<^sub>1 = a # w\<^sub>2 \<and> map Old_sym \<alpha>\<^sub>2 = map Old_sym \<beta> @ map Old_sym \<alpha> \<and> 
+                    (Old_st p\<^sub>2, map Old_sym \<beta>) \<in> trans_fun final_to_stack_pda (Old_st p\<^sub>1) a (Old_sym Z))"
     using final_to_stack_pda_trans final_to_stack_pda_eps by fastforce
-  hence "(\<exists>\<beta>. w\<^sub>2 = w\<^sub>1 \<and> map Old_sym \<alpha>\<^sub>2 = \<beta> @ map Old_sym \<alpha>' \<and> (Old_st p\<^sub>2, \<beta>) \<in> eps_fun final_to_stack_pda (Old_st p\<^sub>1) (Old_sym Z')) 
-            \<or> (\<exists>a \<beta>. w\<^sub>1 = a # w\<^sub>2 \<and> map Old_sym \<alpha>\<^sub>2 = \<beta> @ map Old_sym \<alpha>' \<and> (Old_st p\<^sub>2, \<beta>) \<in> trans_fun final_to_stack_pda (Old_st p\<^sub>1) a (Old_sym Z'))"  by blast
-  with \<alpha>\<^sub>1_def show "pda.step\<^sub>1 final_to_stack_pda (Old_st p\<^sub>1, w\<^sub>1, map Old_sym \<alpha>\<^sub>1) (Old_st p\<^sub>2, w\<^sub>2, map Old_sym \<alpha>\<^sub>2)"
+  hence "(\<exists>\<beta>. w\<^sub>2 = w\<^sub>1 \<and> map Old_sym \<alpha>\<^sub>2 = \<beta> @ map Old_sym \<alpha> \<and> (Old_st p\<^sub>2, \<beta>) \<in> eps_fun final_to_stack_pda (Old_st p\<^sub>1) (Old_sym Z)) 
+            \<or> (\<exists>a \<beta>. w\<^sub>1 = a # w\<^sub>2 \<and> map Old_sym \<alpha>\<^sub>2 = \<beta> @ map Old_sym \<alpha> \<and> (Old_st p\<^sub>2, \<beta>) \<in> trans_fun final_to_stack_pda (Old_st p\<^sub>1) a (Old_sym Z))"  by blast
+  with \<alpha>\<^sub>1_def show ?r
     using pda.step\<^sub>1_rule[OF pda_final_to_stack] by simp
 next
-  assume "pda.step\<^sub>1 final_to_stack_pda (Old_st p\<^sub>1, w\<^sub>1, map Old_sym \<alpha>\<^sub>1) (Old_st p\<^sub>2, w\<^sub>2, map Old_sym \<alpha>\<^sub>2)"
-  then obtain Z' \<alpha>' where map_\<alpha>\<^sub>1_def: "map Old_sym \<alpha>\<^sub>1 = Old_sym Z' # map Old_sym \<alpha>'" and rule: 
-        "(\<exists>\<beta>. w\<^sub>2 = w\<^sub>1 \<and> map Old_sym \<alpha>\<^sub>2 = \<beta>@ map Old_sym \<alpha>' \<and> 
-            (Old_st p\<^sub>2, \<beta>) \<in> eps_fun final_to_stack_pda (Old_st p\<^sub>1) (Old_sym Z')) 
-       \<or> (\<exists>a \<beta>. w\<^sub>1 = a # w\<^sub>2 \<and> map Old_sym \<alpha>\<^sub>2 = \<beta>@ map Old_sym \<alpha>' \<and> 
-            (Old_st p\<^sub>2,\<beta>) \<in> trans_fun final_to_stack_pda (Old_st p\<^sub>1) a (Old_sym Z'))"
+  assume ?r
+  then obtain Z \<alpha> where map_\<alpha>\<^sub>1_def: "map Old_sym \<alpha>\<^sub>1 = Old_sym Z # map Old_sym \<alpha>" and rule: 
+        "(\<exists>\<beta>. w\<^sub>2 = w\<^sub>1 \<and> map Old_sym \<alpha>\<^sub>2 = \<beta>@ map Old_sym \<alpha> \<and> 
+            (Old_st p\<^sub>2, \<beta>) \<in> eps_fun final_to_stack_pda (Old_st p\<^sub>1) (Old_sym Z)) 
+       \<or> (\<exists>a \<beta>. w\<^sub>1 = a # w\<^sub>2 \<and> map Old_sym \<alpha>\<^sub>2 = \<beta>@ map Old_sym \<alpha> \<and> 
+            (Old_st p\<^sub>2,\<beta>) \<in> trans_fun final_to_stack_pda (Old_st p\<^sub>1) a (Old_sym Z))"
     using pda.step\<^sub>1_rule_ext[OF pda_final_to_stack] by auto
-  from map_\<alpha>\<^sub>1_def have \<alpha>\<^sub>1_def: "\<alpha>\<^sub>1 = Z' # \<alpha>'"
+  from map_\<alpha>\<^sub>1_def have \<alpha>\<^sub>1_def: "\<alpha>\<^sub>1 = Z # \<alpha>"
     by (metis list.inj_map_strong list.simps(9) sym_extended.inject)
-  from rule have "(\<exists>\<beta>. w\<^sub>2 = w\<^sub>1 \<and> map Old_sym \<alpha>\<^sub>2 = map Old_sym \<beta>@ map Old_sym \<alpha>' \<and> 
-                    (Old_st p\<^sub>2, map Old_sym \<beta>) \<in> eps_fun final_to_stack_pda (Old_st p\<^sub>1) (Old_sym Z')) 
-                \<or> (\<exists>a \<beta>. w\<^sub>1 = a # w\<^sub>2 \<and> map Old_sym \<alpha>\<^sub>2 = map Old_sym \<beta>@ map Old_sym \<alpha>' \<and> 
-                    (Old_st p\<^sub>2, map Old_sym \<beta>) \<in> trans_fun final_to_stack_pda (Old_st p\<^sub>1) a (Old_sym Z'))"
+  from rule have "(\<exists>\<beta>. w\<^sub>2 = w\<^sub>1 \<and> map Old_sym \<alpha>\<^sub>2 = map Old_sym \<beta>@ map Old_sym \<alpha> \<and> 
+                    (Old_st p\<^sub>2, map Old_sym \<beta>) \<in> eps_fun final_to_stack_pda (Old_st p\<^sub>1) (Old_sym Z)) 
+                \<or> (\<exists>a \<beta>. w\<^sub>1 = a # w\<^sub>2 \<and> map Old_sym \<alpha>\<^sub>2 = map Old_sym \<beta>@ map Old_sym \<alpha> \<and> 
+                    (Old_st p\<^sub>2, map Old_sym \<beta>) \<in> trans_fun final_to_stack_pda (Old_st p\<^sub>1) a (Old_sym Z))"
     using append_eq_map_conv[where ?f = Old_sym] by metis
-  hence "(\<exists>\<beta>. w\<^sub>2 = w\<^sub>1 \<and> \<alpha>\<^sub>2 = \<beta>@\<alpha>' \<and> (p\<^sub>2, \<beta>) \<in> eps_fun M p\<^sub>1 Z')
-               \<or> (\<exists>a \<beta>. w\<^sub>1 = a # w\<^sub>2 \<and> \<alpha>\<^sub>2 = \<beta>@\<alpha>' \<and> (p\<^sub>2,\<beta>) \<in> trans_fun M p\<^sub>1 a Z')"
+  hence "(\<exists>\<beta>. w\<^sub>2 = w\<^sub>1 \<and> \<alpha>\<^sub>2 = \<beta>@\<alpha> \<and> (p\<^sub>2, \<beta>) \<in> eps_fun M p\<^sub>1 Z)
+               \<or> (\<exists>a \<beta>. w\<^sub>1 = a # w\<^sub>2 \<and> \<alpha>\<^sub>2 = \<beta>@\<alpha> \<and> (p\<^sub>2,\<beta>) \<in> trans_fun M p\<^sub>1 a Z)"
     using final_to_stack_pda_trans final_to_stack_pda_eps by (metis list.inj_map_strong sym_extended.inject map_append)
-  with \<alpha>\<^sub>1_def show "pda.step\<^sub>1 M (p\<^sub>1, w\<^sub>1, \<alpha>\<^sub>1) (p\<^sub>2, w\<^sub>2, \<alpha>\<^sub>2)"
+  with \<alpha>\<^sub>1_def show ?l
     using step\<^sub>1_rule by simp
 qed
 
-abbreviation "\<alpha>_with_new \<alpha> \<equiv> map Old_sym \<alpha> @ [New_sym]"
+abbreviation \<alpha>_with_new :: "'s list \<Rightarrow> 's sym_extended list" where 
+  "\<alpha>_with_new \<alpha> \<equiv> map Old_sym \<alpha> @ [New_sym]"
 
 lemma final_to_stack_pda_step\<^sub>1_drop:
   assumes "pda.step\<^sub>1 final_to_stack_pda (Old_st p\<^sub>1, w\<^sub>1, \<alpha>_with_new \<alpha>\<^sub>1) 
                                           (Old_st p\<^sub>2, w\<^sub>2, \<alpha>_with_new \<alpha>\<^sub>2)"
     shows "pda.step\<^sub>1 M (p\<^sub>1, w\<^sub>1, \<alpha>\<^sub>1) (p\<^sub>2, w\<^sub>2, \<alpha>\<^sub>2)"
 proof -
-  from assms obtain Z' \<alpha>' where map_\<alpha>\<^sub>1_def: "\<alpha>_with_new \<alpha>\<^sub>1 = Z' # \<alpha>'" and rule: 
-      "(\<exists>\<beta>. w\<^sub>2 = w\<^sub>1 \<and> \<alpha>_with_new \<alpha>\<^sub>2 = \<beta>@\<alpha>' \<and> (Old_st p\<^sub>2, \<beta>) \<in> final_to_stack_eps_fun (Old_st p\<^sub>1) Z') 
-          \<or> (\<exists>a \<beta>. w\<^sub>1 = a # w\<^sub>2 \<and> \<alpha>_with_new \<alpha>\<^sub>2 = \<beta>@\<alpha>' \<and> (Old_st p\<^sub>2,\<beta>) \<in> final_to_stack_trans_fun (Old_st p\<^sub>1) a Z')"
+  from assms obtain Z \<alpha> where \<alpha>\<^sub>1_with_new_def: "\<alpha>_with_new \<alpha>\<^sub>1 = Z # \<alpha>" and rule: 
+      "(\<exists>\<beta>. w\<^sub>2 = w\<^sub>1 \<and> \<alpha>_with_new \<alpha>\<^sub>2 = \<beta>@\<alpha> \<and> (Old_st p\<^sub>2, \<beta>) \<in> final_to_stack_eps_fun (Old_st p\<^sub>1) Z) 
+          \<or> (\<exists>a \<beta>. w\<^sub>1 = a # w\<^sub>2 \<and> \<alpha>_with_new \<alpha>\<^sub>2 = \<beta>@\<alpha> \<and> (Old_st p\<^sub>2,\<beta>) \<in> final_to_stack_trans_fun (Old_st p\<^sub>1) a Z)"
     using pda.step\<^sub>1_rule_ext[OF pda_final_to_stack] by (auto simp: final_to_stack_pda_def)
-  hence "Z' \<noteq> New_sym"
-    by (induction "Old_st p\<^sub>1" Z' rule: final_to_stack_eps_fun.induct) (auto, metis empty_iff fst_conv singletonD st_extended.simps(5))
-  with map_\<alpha>\<^sub>1_def have "map Old_sym \<alpha>\<^sub>1 \<noteq> []" by auto
+  from rule have "Z \<noteq> New_sym"
+    by (induction "Old_st p\<^sub>1" Z rule: final_to_stack_eps_fun.induct) (auto, metis empty_iff fst_conv singletonD st_extended.simps(5))
+  with \<alpha>\<^sub>1_with_new_def have "map Old_sym \<alpha>\<^sub>1 \<noteq> []" by auto
   with assms have "pda.step\<^sub>1 final_to_stack_pda (Old_st p\<^sub>1, w\<^sub>1, map Old_sym \<alpha>\<^sub>1) 
                                             (Old_st p\<^sub>2, w\<^sub>2, map Old_sym \<alpha>\<^sub>2)"
     using pda.step\<^sub>1_stack_drop[OF pda_final_to_stack] by blast
@@ -155,57 +137,33 @@ lemma final_to_stack_pda_from_old:
   assumes "pda.step\<^sub>1 final_to_stack_pda (Old_st p\<^sub>1, w\<^sub>1, \<alpha>\<^sub>1) (p\<^sub>2, w\<^sub>2, \<alpha>\<^sub>2)"
     shows "(\<exists>p\<^sub>2'. p\<^sub>2 = Old_st p\<^sub>2') \<or> p\<^sub>2 = New_final"
 proof -
-  from assms obtain Z' \<alpha>' where "\<alpha>\<^sub>1 = Z'#\<alpha>'" and rule: 
-        "(\<exists>\<beta>. w\<^sub>2 = w\<^sub>1 \<and> \<alpha>\<^sub>2 = \<beta>@\<alpha>' \<and> (p\<^sub>2, \<beta>) \<in> final_to_stack_eps_fun (Old_st p\<^sub>1) Z') 
-            \<or> (\<exists>a \<beta>. w\<^sub>1 = a # w\<^sub>2 \<and> \<alpha>\<^sub>2 = \<beta>@\<alpha>' \<and> (p\<^sub>2,\<beta>) \<in> final_to_stack_trans_fun (Old_st p\<^sub>1) a Z')"
-    using pda.step\<^sub>1_rule_ext[OF pda_final_to_stack] by (auto simp: final_to_stack_pda_def)
+  from assms obtain Z \<alpha> where rule: 
+        "(\<exists>\<beta>. w\<^sub>2 = w\<^sub>1 \<and> \<alpha>\<^sub>2 = \<beta>@\<alpha> \<and> (p\<^sub>2, \<beta>) \<in> final_to_stack_eps_fun (Old_st p\<^sub>1) Z) 
+            \<or> (\<exists>a \<beta>. w\<^sub>1 = a # w\<^sub>2 \<and> \<alpha>\<^sub>2 = \<beta>@\<alpha> \<and> (p\<^sub>2,\<beta>) \<in> final_to_stack_trans_fun (Old_st p\<^sub>1) a Z)"
+    using pda.step\<^sub>1_rule_ext[OF pda_final_to_stack] by (auto simp: final_to_stack_pda_def)+
   thus ?thesis 
-    by (induction "Old_st p\<^sub>1" Z' rule: final_to_stack_eps_fun.induct, auto) (metis empty_iff fst_conv singletonD)+
+    by (induction "Old_st p\<^sub>1" Z rule: final_to_stack_eps_fun.induct, auto) (metis empty_iff fst_conv singletonD)+
 qed
 
 lemma final_to_stack_pda_from_final:
-  assumes "pda.step\<^sub>1 final_to_stack_pda (New_final :: 'q st_extended, w\<^sub>1, \<alpha>\<^sub>1) (p\<^sub>2, w\<^sub>2, \<alpha>\<^sub>2)"
+  assumes "pda.step\<^sub>1 final_to_stack_pda (New_final, w\<^sub>1, \<alpha>\<^sub>1) (p\<^sub>2, w\<^sub>2, \<alpha>\<^sub>2)"
     shows "\<exists>Z'. p\<^sub>2 = New_final \<and> w\<^sub>2 = w\<^sub>1 \<and> \<alpha>\<^sub>1 = Z'#\<alpha>\<^sub>2"
 proof -
-  from assms obtain Z' \<alpha>' where \<alpha>\<^sub>1_def: "\<alpha>\<^sub>1 = Z'#\<alpha>'" and rule: 
-        "(\<exists>\<beta>. w\<^sub>2 = w\<^sub>1 \<and> \<alpha>\<^sub>2 = \<beta>@\<alpha>' \<and> (p\<^sub>2,\<beta>) \<in> final_to_stack_eps_fun New_final Z') 
-          \<or> (\<exists>a \<beta>. w\<^sub>1 = a # w\<^sub>2 \<and> \<alpha>\<^sub>2 = \<beta>@\<alpha>' \<and> (p\<^sub>2,\<beta>) \<in> final_to_stack_trans_fun New_final a Z')"
+  from assms obtain Z \<alpha> where \<alpha>\<^sub>1_def: "\<alpha>\<^sub>1 = Z#\<alpha>" and rule: 
+        "(\<exists>\<beta>. w\<^sub>2 = w\<^sub>1 \<and> \<alpha>\<^sub>2 = \<beta>@\<alpha> \<and> (p\<^sub>2,\<beta>) \<in> final_to_stack_eps_fun New_final Z) 
+          \<or> (\<exists>a \<beta>. w\<^sub>1 = a # w\<^sub>2 \<and> \<alpha>\<^sub>2 = \<beta>@\<alpha> \<and> (p\<^sub>2,\<beta>) \<in> final_to_stack_trans_fun New_final a Z)"
     using pda.step\<^sub>1_rule_ext[OF pda_final_to_stack] by (auto simp: final_to_stack_pda_def)
   thus ?thesis 
-    by (induction "New_final:: 'q st_extended" Z' rule: final_to_stack_eps_fun.induct) auto
+    by (induction "New_final:: 'q st_extended" Z rule: final_to_stack_eps_fun.induct) auto
 qed
-
-lemma final_to_stack_pda_from_finaln:
-  assumes "pda.steps final_to_stack_pda (New_final :: 'q st_extended, w\<^sub>1, \<alpha>\<^sub>1) (p\<^sub>2, w\<^sub>2, \<alpha>\<^sub>2)"
-  shows "\<exists>\<gamma>. p\<^sub>2 = New_final \<and> w\<^sub>2 = w\<^sub>1 \<and> \<alpha>\<^sub>1 = \<gamma>@\<alpha>\<^sub>2"
-using assms proof (induction "(New_final :: 'q st_extended, w\<^sub>1, \<alpha>\<^sub>1)" "(p\<^sub>2, w\<^sub>2, \<alpha>\<^sub>2)" 
-                     arbitrary: w\<^sub>1 \<alpha>\<^sub>1 rule: pda.steps_induct[OF pda_final_to_stack])
-  case (3 w\<^sub>1 \<alpha>\<^sub>1 p' w' \<alpha>')
-  from 3(1) obtain Z' where p'_final: "p' = New_final" and w_eq: "w' = w\<^sub>1" and \<alpha>\<^sub>1_def: "\<alpha>\<^sub>1 = Z'#\<alpha>'"
-    using final_to_stack_pda_from_final by blast
-  with 3(2,3) obtain \<gamma> where "p\<^sub>2 = New_final" and "w\<^sub>2 = w'" and "\<alpha>' = \<gamma> @ \<alpha>\<^sub>2" by blast
-  with w_eq \<alpha>\<^sub>1_def show ?case by auto
-qed (simp_all add: assms)
 
 lemma final_to_stack_pda_from_oldn:
   assumes "pda.steps final_to_stack_pda (Old_st p\<^sub>1, w\<^sub>1, \<alpha>\<^sub>1) (p\<^sub>2, w\<^sub>2, \<alpha>\<^sub>2)"
   shows "\<exists>q'. p\<^sub>2 = Old_st q' \<or> p\<^sub>2 = New_final"
-  using assms proof (induction "(Old_st p\<^sub>1, w\<^sub>1, \<alpha>\<^sub>1)" "(p\<^sub>2, w\<^sub>2, \<alpha>\<^sub>2)" 
-                      arbitrary: p\<^sub>1 w\<^sub>1 \<alpha>\<^sub>1 rule: pda.steps_induct[OF pda_final_to_stack])
-  case (3 w\<^sub>1 \<alpha>\<^sub>1 p' w' \<alpha>')
-  from 3(1) have case_dist: "(\<exists>p''. p' = Old_st p'') \<or> p' = New_final"
-    using final_to_stack_pda_from_old by simp
-  then show ?case proof (cases)
-    assume "\<exists>p''. p' = Old_st p''"
-    then obtain p'' where "p' = Old_st p''" by blast
-    with 3(2,3) show ?case by auto
-  next
-    assume "\<not>(\<exists>p''. p' = Old_st p'')"
-    with case_dist have "p' = New_final" by blast
-    with 3(2) show ?case
-      using final_to_stack_pda_from_finaln by blast
-  qed
-qed (auto simp: assms)
+  apply (induction "(Old_st p\<^sub>1, w\<^sub>1, \<alpha>\<^sub>1)" "(p\<^sub>2, w\<^sub>2, \<alpha>\<^sub>2)" arbitrary: p\<^sub>2 w\<^sub>2 \<alpha>\<^sub>2 rule: pda.steps_induct2[OF pda_final_to_stack])
+    apply (auto simp: assms)
+  apply (use final_to_stack_pda_from_old final_to_stack_pda_from_final in blast)+
+  done
 
 lemma final_to_stack_pda_to_old:
   assumes "pda.step\<^sub>1 final_to_stack_pda (p\<^sub>1, w\<^sub>1, \<alpha>\<^sub>1) (Old_st p\<^sub>2, w\<^sub>2, \<alpha>\<^sub>2)"
@@ -214,46 +172,33 @@ using assms final_to_stack_pda_from_final by (metis st_extended.exhaust)
 
 lemma final_to_stack_pda_bottom_elem:
   assumes "pda.steps final_to_stack_pda (Old_st p\<^sub>1, w\<^sub>1, \<alpha>_with_new \<alpha>\<^sub>1) (Old_st p\<^sub>2, w\<^sub>2, \<gamma>)"
-    shows "\<exists>\<alpha>. \<gamma> = \<alpha>_with_new \<alpha>"
-proof -
-  from assms obtain n where stepn: "pda.stepn final_to_stack_pda n (Old_st p\<^sub>1, w\<^sub>1, \<alpha>_with_new \<alpha>\<^sub>1) (Old_st p\<^sub>2, w\<^sub>2, \<gamma>)"
-    using pda.stepn_steps[OF pda_final_to_stack] by blast
-  thus ?thesis proof 
-   (induction n "(Old_st p\<^sub>1, w\<^sub>1, \<alpha>_with_new \<alpha>\<^sub>1)" "(Old_st p\<^sub>2, w\<^sub>2, \<gamma>)"
-       arbitrary: p\<^sub>2 w\<^sub>2 \<gamma> rule: pda.stepn.induct[OF pda_final_to_stack])
-    case (3 n p\<^sub>2 w\<^sub>2 \<alpha>\<^sub>2 w\<^sub>3 \<alpha>\<^sub>3 p\<^sub>3)
-    from 3(1) have steps: "pda.steps final_to_stack_pda (Old_st p\<^sub>1, w\<^sub>1, \<alpha>_with_new \<alpha>\<^sub>1) (p\<^sub>2, w\<^sub>2, \<alpha>\<^sub>2)"
-      using pda.stepn_steps[OF pda_final_to_stack] by blast
-    obtain p\<^sub>2' where p\<^sub>2_def: "p\<^sub>2 = Old_st p\<^sub>2'"
-      using final_to_stack_pda_from_oldn[OF steps] final_to_stack_pda_to_old[OF 3(3)] by blast
-    with 3(1,2) have \<alpha>\<^sub>2_def: "\<exists>\<alpha>. \<alpha>\<^sub>2 = \<alpha>_with_new \<alpha>" by simp
-    from p\<^sub>2_def 3(3) obtain Z' \<alpha>' where \<alpha>\<^sub>2_split: "\<alpha>\<^sub>2 = Z' # \<alpha>'" and rule:
-    "(\<exists>\<beta>. w\<^sub>3 = w\<^sub>2 \<and> \<alpha>\<^sub>3 = \<beta> @ \<alpha>' \<and> (Old_st p\<^sub>3, \<beta>) \<in> final_to_stack_eps_fun (Old_st p\<^sub>2') Z') 
-     \<or> (\<exists>a \<beta>. w\<^sub>2 = a # w\<^sub>3 \<and> \<alpha>\<^sub>3 = \<beta> @ \<alpha>' \<and> (Old_st p\<^sub>3, \<beta>) \<in> final_to_stack_trans_fun (Old_st p\<^sub>2') a Z')"
-      using pda.step\<^sub>1_rule_ext[OF pda_final_to_stack] by (auto simp: final_to_stack_pda_def)
-    hence "\<exists>Z. Z' = Old_sym Z"
-      by (induction "Old_st p\<^sub>2'" Z' rule: final_to_stack_eps_fun.induct) 
-            (auto, meson empty_iff insert_iff prod.inject st_extended.distinct(3))
-    with \<alpha>\<^sub>2_def \<alpha>\<^sub>2_split have "\<exists>\<gamma>. \<alpha>' = \<alpha>_with_new \<gamma>"
-      by (metis hd_append list.sel(1,3) map_tl sym_extended.simps(3) tl_append_if)
-    with rule show ?case
-      by (induction "Old_st p\<^sub>2'" Z' rule: final_to_stack_eps_fun.induct, auto)
-          (metis empty_iff fst_conv singleton_iff st_extended.distinct(3), metis map_append,
-                  metis map_append, metis empty_iff fst_conv singleton_iff st_extended.distinct(3))
-  qed (auto simp: stepn)
-qed
+  shows "\<exists>\<alpha>. \<gamma> = \<alpha>_with_new \<alpha>"
+proof (induction "(Old_st p\<^sub>1, w\<^sub>1, \<alpha>_with_new \<alpha>\<^sub>1)" "(Old_st p\<^sub>2, w\<^sub>2, \<gamma>)" arbitrary: p\<^sub>2 w\<^sub>2 \<gamma> rule: pda.steps_induct2[OF pda_final_to_stack])
+  case (3 p\<^sub>2 w\<^sub>2 \<alpha>\<^sub>2 w\<^sub>3 \<alpha>\<^sub>3 p\<^sub>3)
+  obtain p\<^sub>2' where p\<^sub>2_def: "p\<^sub>2 = Old_st p\<^sub>2'"
+    using final_to_stack_pda_from_oldn[OF 3(1)] final_to_stack_pda_to_old[OF 3(2)] by blast
+  with 3(3) have \<alpha>\<^sub>2_def: "\<exists>\<alpha>. \<alpha>\<^sub>2 = \<alpha>_with_new \<alpha>" by simp
+  from p\<^sub>2_def 3(2) obtain Z \<alpha> where \<alpha>\<^sub>2_split: "\<alpha>\<^sub>2 = Z # \<alpha>" and rule:
+    "(\<exists>\<beta>. w\<^sub>3 = w\<^sub>2 \<and> \<alpha>\<^sub>3 = \<beta> @ \<alpha> \<and> (Old_st p\<^sub>3, \<beta>) \<in> final_to_stack_eps_fun (Old_st p\<^sub>2') Z) 
+     \<or> (\<exists>a \<beta>. w\<^sub>2 = a # w\<^sub>3 \<and> \<alpha>\<^sub>3 = \<beta> @ \<alpha> \<and> (Old_st p\<^sub>3, \<beta>) \<in> final_to_stack_trans_fun (Old_st p\<^sub>2') a Z)"
+    using pda.step\<^sub>1_rule_ext[OF pda_final_to_stack] by (auto simp: final_to_stack_pda_def)
+  hence "\<exists>Z'. Z = Old_sym Z'"
+    by (induction "Old_st p\<^sub>2'" Z rule: final_to_stack_eps_fun.induct) 
+          (auto, meson empty_iff insert_iff prod.inject st_extended.distinct(3))
+  with \<alpha>\<^sub>2_def \<alpha>\<^sub>2_split have "\<exists>\<gamma>. \<alpha> = \<alpha>_with_new \<gamma>"
+    by (metis hd_append list.sel(1,3) map_tl sym_extended.simps(3) tl_append_if)
+  with rule show ?case
+    by (induction "Old_st p\<^sub>2'" Z rule: final_to_stack_eps_fun.induct, auto)
+        (metis empty_iff fst_conv singleton_iff st_extended.distinct(3), metis map_append,
+           metis map_append, metis empty_iff fst_conv singleton_iff st_extended.distinct(3))
+qed (auto simp: assms)
 
 lemma final_to_stack_pda_stepn:
   "pda.stepn M n (p\<^sub>1, w\<^sub>1, \<alpha>\<^sub>1) (p\<^sub>2, w\<^sub>2, \<alpha>\<^sub>2) \<longleftrightarrow> 
-      pda.stepn final_to_stack_pda n (Old_st p\<^sub>1, w\<^sub>1, \<alpha>_with_new \<alpha>\<^sub>1) (Old_st p\<^sub>2, w\<^sub>2, \<alpha>_with_new \<alpha>\<^sub>2)"
+      pda.stepn final_to_stack_pda n (Old_st p\<^sub>1, w\<^sub>1, \<alpha>_with_new \<alpha>\<^sub>1) (Old_st p\<^sub>2, w\<^sub>2, \<alpha>_with_new \<alpha>\<^sub>2)" (is "?l \<longleftrightarrow> ?r")
 proof
-  assume asm: "pda.stepn M n (p\<^sub>1, w\<^sub>1, \<alpha>\<^sub>1) (p\<^sub>2, w\<^sub>2, \<alpha>\<^sub>2)"
-  thus "pda.stepn final_to_stack_pda n (Old_st p\<^sub>1, w\<^sub>1, \<alpha>_with_new \<alpha>\<^sub>1) (Old_st p\<^sub>2, w\<^sub>2, \<alpha>_with_new \<alpha>\<^sub>2)"
+  show "?l \<Longrightarrow> ?r"
   proof (induction n "(p\<^sub>1, w\<^sub>1, \<alpha>\<^sub>1)" "(p\<^sub>2, w\<^sub>2, \<alpha>\<^sub>2)" arbitrary: p\<^sub>2 w\<^sub>2 \<alpha>\<^sub>2 rule: stepn.induct)
-    case refl\<^sub>n
-    then show ?case
-      by (simp add: pda.refl\<^sub>n[OF pda_final_to_stack])
-  next
     case (step\<^sub>n n p\<^sub>2 w\<^sub>2 \<alpha>\<^sub>2 p\<^sub>3 w\<^sub>3 \<alpha>\<^sub>3)
     from step\<^sub>n(3) have "pda.step\<^sub>1 final_to_stack_pda (Old_st p\<^sub>2, w\<^sub>2, map Old_sym \<alpha>\<^sub>2) (Old_st p\<^sub>3, w\<^sub>3, map Old_sym \<alpha>\<^sub>3)"
       using final_to_stack_pda_step by simp
@@ -261,29 +206,26 @@ proof
       using pda.step\<^sub>1_stack_app[OF pda_final_to_stack] by simp
     with step\<^sub>n(2) show ?case
       by (simp add: pda.step\<^sub>n[OF pda_final_to_stack])
-  qed
+  qed (simp add: pda.refl\<^sub>n[OF pda_final_to_stack])
 next
-  assume asm: "pda.stepn final_to_stack_pda n (Old_st p\<^sub>1, w\<^sub>1, \<alpha>_with_new \<alpha>\<^sub>1) (Old_st p\<^sub>2, w\<^sub>2, \<alpha>_with_new \<alpha>\<^sub>2)"
-  thus "pda.stepn M n (p\<^sub>1, w\<^sub>1, \<alpha>\<^sub>1) (p\<^sub>2, w\<^sub>2, \<alpha>\<^sub>2)"
+  assume r: ?r thus ?l
   proof (induction n "(Old_st p\<^sub>1, w\<^sub>1, \<alpha>_with_new \<alpha>\<^sub>1)" "(Old_st p\<^sub>2, w\<^sub>2, \<alpha>_with_new \<alpha>\<^sub>2)" 
                  arbitrary: p\<^sub>2 w\<^sub>2 \<alpha>\<^sub>2 rule: pda.stepn.induct[OF pda_final_to_stack])
-    case 2
-    from 2(1) have "\<alpha>\<^sub>1 = \<alpha>\<^sub>2"
-      by (metis list.inj_map_strong sym_extended.inject)
-    thus ?case by simp
-  next
     case (3 n p\<^sub>2 w\<^sub>2 \<alpha>\<^sub>2 w\<^sub>3 p\<^sub>3 \<alpha>\<^sub>3)
-    from 3(1) have steps: "pda.steps final_to_stack_pda (Old_st p\<^sub>1, w\<^sub>1, \<alpha>_with_new \<alpha>\<^sub>1) (p\<^sub>2, w\<^sub>2, \<alpha>\<^sub>2)"
+    from 3(1) have steps_3_1: "pda.steps final_to_stack_pda (Old_st p\<^sub>1, w\<^sub>1, \<alpha>_with_new \<alpha>\<^sub>1) (p\<^sub>2, w\<^sub>2, \<alpha>\<^sub>2)"
       using pda.stepn_steps[OF pda_final_to_stack] by blast
     obtain p\<^sub>2' where p\<^sub>2_def: "p\<^sub>2 = Old_st p\<^sub>2'"
-      using final_to_stack_pda_from_oldn[OF steps] final_to_stack_pda_to_old[OF 3(3)] by blast
-    with steps obtain \<gamma> where \<alpha>\<^sub>2_def: "\<alpha>\<^sub>2 = \<alpha>_with_new \<gamma>"
+      using final_to_stack_pda_from_oldn[OF steps_3_1] final_to_stack_pda_to_old[OF 3(3)] by blast
+    with steps_3_1 obtain \<gamma> where \<alpha>\<^sub>2_def: "\<alpha>\<^sub>2 = \<alpha>_with_new \<gamma>"
       using final_to_stack_pda_bottom_elem by blast
-    with p\<^sub>2_def 3(1,2) have *: "pda.stepn M n (p\<^sub>1, w\<^sub>1, \<alpha>\<^sub>1) (p\<^sub>2', w\<^sub>2, \<gamma>)" by simp
-    from p\<^sub>2_def \<alpha>\<^sub>2_def 3(3) have **: "pda.step\<^sub>1 M (p\<^sub>2', w\<^sub>2, \<gamma>) (p\<^sub>3, w\<^sub>3, \<alpha>\<^sub>3)"
+
+    with p\<^sub>2_def 3(1,2) have "pda.stepn M n (p\<^sub>1, w\<^sub>1, \<alpha>\<^sub>1) (p\<^sub>2', w\<^sub>2, \<gamma>)" by simp
+
+    moreover from p\<^sub>2_def \<alpha>\<^sub>2_def 3(3) have "pda.step\<^sub>1 M (p\<^sub>2', w\<^sub>2, \<gamma>) (p\<^sub>3, w\<^sub>3, \<alpha>\<^sub>3)"
       using final_to_stack_pda_step\<^sub>1_drop by simp
-    from * ** show ?case by simp
-  qed (simp add: asm)
+
+    ultimately show ?case by simp
+  qed (rule r, metis refl\<^sub>n list.inj_map_strong sym_extended.inject)
 qed
 
 lemma final_to_stack_pda_steps:
@@ -294,48 +236,27 @@ using final_to_stack_pda_stepn pda.stepn_steps[OF pda_final_to_stack] stepn_step
 lemma final_to_stack_pda_final_dump:
   "pda.steps final_to_stack_pda (New_final, w, \<gamma>) (New_final, w, [])"
 proof (induction \<gamma>)
-  case Nil
-  then show ?case
-    by (simp add: pda.steps_refl[OF pda_final_to_stack])
-next
   case (Cons Z \<gamma>)
   have "(New_final, []) \<in> final_to_stack_eps_fun New_final Z" by simp
   hence "pda.step\<^sub>1 final_to_stack_pda (New_final, w, Z # \<gamma>) (New_final, w, \<gamma>)"
     using pda.step\<^sub>1_rule[OF pda_final_to_stack] by (simp add: final_to_stack_pda_def)
   with Cons.IH show ?case
-    using pda.step\<^sub>1_stepn_one[OF pda_final_to_stack] pda.stepn_steps[OF pda_final_to_stack] 
-          pda.steps_trans[OF pda_final_to_stack] by metis
-qed
+    using pda.step\<^sub>1_steps[OF pda_final_to_stack] pda.steps_trans[OF pda_final_to_stack] by blast
+qed (simp add: pda.steps_refl[OF pda_final_to_stack])
 
 lemma final_to_stack_pda_first_step:
   assumes "pda.step\<^sub>1 final_to_stack_pda (New_init, w\<^sub>1, [New_sym]) (p\<^sub>2, w\<^sub>2, \<alpha>)"
-    shows "p\<^sub>2 = Old_st (init_state M) \<and> w\<^sub>2 = w\<^sub>1 \<and> \<alpha> = [Old_sym (init_symbol M), New_sym]"
-proof -
-  from assms have "(\<exists>\<beta>. w\<^sub>2 = w\<^sub>1 \<and> \<alpha> = \<beta> \<and> (p\<^sub>2, \<beta>) \<in> final_to_stack_eps_fun New_init New_sym) 
-                   \<or> (\<exists>a \<beta>. w\<^sub>1 = a # w\<^sub>2 \<and> \<alpha> = \<beta> \<and> (p\<^sub>2, \<beta>) \<in> final_to_stack_trans_fun New_init a New_sym)"
-    using pda.step\<^sub>1_rule[OF pda_final_to_stack] by (simp add: final_to_stack_pda_def)
-  thus ?thesis by simp
-qed
+  shows "p\<^sub>2 = Old_st (init_state M) \<and> w\<^sub>2 = w\<^sub>1 \<and> \<alpha> = [Old_sym (init_symbol M), New_sym]"
+using assms pda.step\<^sub>1_rule[OF pda_final_to_stack] by (simp add: final_to_stack_pda_def)
 
 lemma final_to_stack_pda_empty_only_final:
   assumes "pda.steps final_to_stack_pda (New_init, w\<^sub>1, [New_sym]) (q, w\<^sub>2, [])"
-    shows "q = New_final"
+  shows "q = New_final"
 proof -
-  from assms obtain n where stepn: "pda.stepn final_to_stack_pda n (New_init, w\<^sub>1, [New_sym]) (q, w\<^sub>2, [])"
-    using pda.stepn_steps[OF pda_final_to_stack] by blast
-  then obtain n' where "n = Suc n'"
-    using pda.stepn_not_refl[OF pda_final_to_stack] gr0_implies_Suc by blast
-  with stepn have "pda.stepn final_to_stack_pda n'
-                              (Old_st (init_state M), w\<^sub>1, [Old_sym (init_symbol M), New_sym])
-                              (q, w\<^sub>2, [])"
-    using pda.stepn_split_first[OF pda_final_to_stack] final_to_stack_pda_first_step by blast
-  hence steps: "pda.steps final_to_stack_pda (Old_st (init_state M), w\<^sub>1, [Old_sym (init_symbol M), New_sym])
-                                            (q, w\<^sub>2, [])"
-    using pda.stepn_steps[OF pda_final_to_stack] by blast
-  hence case_dist: "\<exists>q'. q = Old_st q' \<or> q = New_final"
-    using final_to_stack_pda_from_oldn by blast
-  with steps show ?thesis
-    using final_to_stack_pda_bottom_elem[of "init_state M" w\<^sub>1 "[init_symbol M]" _ w\<^sub>2 "[]"] by auto
+  from assms have "pda.steps final_to_stack_pda (Old_st (init_state M), w\<^sub>1, [Old_sym (init_symbol M), New_sym]) (q, w\<^sub>2, [])"
+    using pda.steps_not_refl_split_first[OF pda_final_to_stack] final_to_stack_pda_first_step by blast
+  thus ?thesis
+    using final_to_stack_pda_bottom_elem[of "init_state M" w\<^sub>1 "[init_symbol M]" _ w\<^sub>2 "[]"]  final_to_stack_pda_from_oldn by fastforce
 qed
 
 lemma final_to_stack_pda_split_old_final:
@@ -351,19 +272,24 @@ using assms proof (induction "Suc n" "(Old_st p\<^sub>1, w\<^sub>1, \<alpha>\<^s
     case 0
     with 3(1) have p\<^sub>2_def: "Old_st p\<^sub>1 = p\<^sub>2" and w12: "w\<^sub>1 = w\<^sub>2" and a12: "\<alpha>\<^sub>1 = \<alpha>\<^sub>2"
       using pda.stepn_zeroE[OF pda_final_to_stack] by blast+
-    from p\<^sub>2_def 3(3) obtain Z' \<alpha>' where \<alpha>\<^sub>2_def: "\<alpha>\<^sub>2 = Z' # \<alpha>'" and rule: 
-            "(\<exists>\<beta>. w\<^sub>3 = w\<^sub>2 \<and> \<alpha>\<^sub>3 = \<beta>@\<alpha>' \<and> (New_final,\<beta>) \<in> final_to_stack_eps_fun (Old_st p\<^sub>1) Z') 
-               \<or> (\<exists>a \<beta>. w\<^sub>2 = a # w\<^sub>3 \<and> \<alpha>\<^sub>3 = \<beta>@\<alpha>' \<and> (New_final,\<beta>) \<in> final_to_stack_trans_fun (Old_st p\<^sub>1) a Z')"
+    from p\<^sub>2_def 3(3) obtain Z \<alpha> where \<alpha>\<^sub>2_def: "\<alpha>\<^sub>2 = Z # \<alpha>" and rule: 
+            "(\<exists>\<beta>. w\<^sub>3 = w\<^sub>2 \<and> \<alpha>\<^sub>3 = \<beta>@\<alpha> \<and> (New_final,\<beta>) \<in> final_to_stack_eps_fun (Old_st p\<^sub>1) Z) 
+               \<or> (\<exists>a \<beta>. w\<^sub>2 = a # w\<^sub>3 \<and> \<alpha>\<^sub>3 = \<beta>@\<alpha> \<and> (New_final,\<beta>) \<in> final_to_stack_trans_fun (Old_st p\<^sub>1) a Z)"
       using pda.step\<^sub>1_rule_ext[OF pda_final_to_stack] by (auto simp: final_to_stack_pda_def)
     from \<alpha>\<^sub>2_def rule have p\<^sub>1_final: "p\<^sub>1 \<in> final_states M" and w23: "w\<^sub>3 = w\<^sub>2" and a23: "\<alpha>\<^sub>3 = \<alpha>\<^sub>2"
-      by (induction "Old_st p\<^sub>1" Z' rule: final_to_stack_eps_fun.induct, auto)
+      by (induction "Old_st p\<^sub>1" Z rule: final_to_stack_eps_fun.induct, auto)
          (meson empty_iff, meson empty_iff prod.inject singletonD, meson empty_iff, meson empty_iff prod.inject singletonD)
-    from w12 w23 a12 a23 have *: "pda.stepn final_to_stack_pda 0 (Old_st p\<^sub>1, w\<^sub>1, \<alpha>\<^sub>1) (Old_st p\<^sub>1, w\<^sub>3, \<alpha>\<^sub>3)"
+
+    from w12 w23 a12 a23 have "pda.stepn final_to_stack_pda 0 (Old_st p\<^sub>1, w\<^sub>1, \<alpha>\<^sub>1) (Old_st p\<^sub>1, w\<^sub>3, \<alpha>\<^sub>3)"
       using pda.refl\<^sub>n[OF pda_final_to_stack] by simp
-    from 3(3) p\<^sub>2_def w23 a23 have **: "pda.step\<^sub>1 final_to_stack_pda (Old_st p\<^sub>1, w\<^sub>3, \<alpha>\<^sub>3) (New_final, w\<^sub>3, \<alpha>\<^sub>3)" by simp
-    from 0 have ***: "pda.stepn final_to_stack_pda (n - 0) (New_final, w\<^sub>3, \<alpha>\<^sub>3) (New_final, w\<^sub>3, \<alpha>\<^sub>3)"
+
+    moreover from 3(3) p\<^sub>2_def w23 a23 have "pda.step\<^sub>1 final_to_stack_pda (Old_st p\<^sub>1, w\<^sub>3, \<alpha>\<^sub>3) (New_final, w\<^sub>3, \<alpha>\<^sub>3)" by simp
+
+    moreover from 0 have "pda.stepn final_to_stack_pda (n - 0) (New_final, w\<^sub>3, \<alpha>\<^sub>3) (New_final, w\<^sub>3, \<alpha>\<^sub>3)"
       using pda.refl\<^sub>n[OF pda_final_to_stack] by simp
-    from p\<^sub>1_final * ** *** show ?thesis by blast
+
+    ultimately show ?thesis 
+      using p\<^sub>1_final by blast
   next
     case (Suc n')
     then show ?thesis proof (cases "p\<^sub>2 = New_final")
@@ -378,13 +304,18 @@ using assms proof (induction "Suc n" "(Old_st p\<^sub>1, w\<^sub>1, \<alpha>\<^s
         using pda.step\<^sub>1_rule_ext[OF pda_final_to_stack] by (auto simp: final_to_stack_pda_def)
       from rule have w23: "w\<^sub>3 = w\<^sub>2"
         by (induction "New_final :: 'q st_extended" Z' rule: final_to_stack_eps_fun.induct) auto
-      from k_less Suc have *: "k \<le> n" by simp
-      from stepn w23 have **: "pda.stepn final_to_stack_pda k (Old_st p\<^sub>1, w\<^sub>1, \<alpha>\<^sub>1) (Old_st q, w\<^sub>3, \<gamma>)" by simp
-      from step1 w23 have ***: "pda.step\<^sub>1 final_to_stack_pda (Old_st q, w\<^sub>3, \<gamma>) (New_final, w\<^sub>3, \<gamma>)" by simp
-      from stepn' 3(3) True w23 Suc k_less have ****: 
-       "pda.stepn final_to_stack_pda (n - k) (New_final, w\<^sub>3, \<gamma>) (New_final, w\<^sub>3, \<alpha>\<^sub>3)"
+
+      moreover from k_less Suc have "k \<le> n" by simp
+
+      moreover from stepn w23 have "pda.stepn final_to_stack_pda k (Old_st p\<^sub>1, w\<^sub>1, \<alpha>\<^sub>1) (Old_st q, w\<^sub>3, \<gamma>)" by simp
+
+      moreover from step1 w23 have "pda.step\<^sub>1 final_to_stack_pda (Old_st q, w\<^sub>3, \<gamma>) (New_final, w\<^sub>3, \<gamma>)" by simp
+
+      moreover from stepn' 3(3) True w23 Suc k_less have "pda.stepn final_to_stack_pda (n - k) (New_final, w\<^sub>3, \<gamma>) (New_final, w\<^sub>3, \<alpha>\<^sub>3)"
         using pda.step\<^sub>n[OF pda_final_to_stack] by (simp add: Suc_diff_le)
-      from * q_final ** *** **** show ?thesis by blast
+
+      ultimately show ?thesis 
+        using q_final by blast
     next
       case False
       with 3(1) obtain p\<^sub>2' where p\<^sub>2_def: "p\<^sub>2 = Old_st p\<^sub>2'"
@@ -396,11 +327,16 @@ using assms proof (induction "Suc n" "(Old_st p\<^sub>1, w\<^sub>1, \<alpha>\<^s
       hence p\<^sub>2_final: "p\<^sub>2' \<in> final_states M" and w23: "w\<^sub>3 = w\<^sub>2" and a23: "\<alpha>\<^sub>3 = \<alpha>\<^sub>2"
         by (induction "Old_st p\<^sub>2'" Z' rule: final_to_stack_eps_fun.induct, auto)
           (meson empty_iff, meson empty_iff prod.inject singletonD, meson empty_iff, meson empty_iff prod.inject singletonD)
-      from 3(1) p\<^sub>2_def w23 a23 have *: "pda.stepn final_to_stack_pda n (Old_st p\<^sub>1, w\<^sub>1, \<alpha>\<^sub>1) (Old_st p\<^sub>2', w\<^sub>3, \<alpha>\<^sub>3)" by simp
-      from 3(3) p\<^sub>2_def w23 a23 have **: "pda.step\<^sub>1 final_to_stack_pda (Old_st p\<^sub>2', w\<^sub>3, \<alpha>\<^sub>3) (New_final, w\<^sub>3, \<alpha>\<^sub>3)" by simp
-      have ***: "pda.stepn final_to_stack_pda 0 (New_final, w\<^sub>3, \<alpha>\<^sub>3) (New_final, w\<^sub>3, \<alpha>\<^sub>3)"
+
+      from 3(1) p\<^sub>2_def w23 a23 have "pda.stepn final_to_stack_pda n (Old_st p\<^sub>1, w\<^sub>1, \<alpha>\<^sub>1) (Old_st p\<^sub>2', w\<^sub>3, \<alpha>\<^sub>3)" by simp
+
+      moreover from 3(3) p\<^sub>2_def w23 a23 have "pda.step\<^sub>1 final_to_stack_pda (Old_st p\<^sub>2', w\<^sub>3, \<alpha>\<^sub>3) (New_final, w\<^sub>3, \<alpha>\<^sub>3)" by simp
+
+      moreover have "pda.stepn final_to_stack_pda 0 (New_final, w\<^sub>3, \<alpha>\<^sub>3) (New_final, w\<^sub>3, \<alpha>\<^sub>3)"
         using pda.refl\<^sub>n[OF pda_final_to_stack] by simp
-      from p\<^sub>2_final * ** *** show ?thesis by force
+
+      ultimately show ?thesis 
+        using p\<^sub>2_final by force
     qed
   qed
 qed (simp add: assms)
@@ -431,53 +367,54 @@ qed
 
 lemma final_to_stack_pda_path_length:
   assumes "pda.stepn final_to_stack_pda n (New_init, w\<^sub>1, [New_sym]) (New_final, w\<^sub>2, \<gamma>)"
-    shows "n \<ge> 2"
+    shows "\<exists>n'. n = Suc (Suc n')"
 proof -
-  from assms obtain n' where n_def: "n = Suc n'"
-    using pda.stepn_not_refl[OF pda_final_to_stack] gr0_implies_Suc by blast
-  with assms have "pda.stepn final_to_stack_pda n' (Old_st (init_state M), w\<^sub>1, [Old_sym (init_symbol M), New_sym])
-                                                       (New_final, w\<^sub>2, \<gamma>)"
-    using pda.stepn_split_first[OF pda_final_to_stack] final_to_stack_pda_first_step by blast
-  then obtain n'' where "n' = Suc n''"
-    using pda.stepn_not_refl[OF pda_final_to_stack] gr0_implies_Suc by blast
+  from assms obtain n' where n_def: "n = Suc n'" and 
+            stepn': "pda.stepn final_to_stack_pda n' (Old_st (init_state M), w\<^sub>1, [Old_sym (init_symbol M), New_sym])
+                                              (New_final, w\<^sub>2, \<gamma>)"
+    using pda.stepn_not_refl_split_first[OF pda_final_to_stack] final_to_stack_pda_first_step by blast
+  from stepn' obtain n'' where "n' = Suc n''"
+    using pda.stepn_not_refl_split_first[OF pda_final_to_stack] by blast
   with n_def show ?thesis by simp
 qed
 
 lemma accepted_final_to_stack:
 "(\<exists>q \<gamma>. q \<in> final_states M \<and> pda.steps M (init_state M, w, [init_symbol M]) (q, [], \<gamma>)) \<longleftrightarrow>
-  (\<exists>q. pda.steps final_to_stack_pda (init_state final_to_stack_pda, w, [init_symbol final_to_stack_pda]) (q, [], []))"
+  (\<exists>q. pda.steps final_to_stack_pda (init_state final_to_stack_pda, w, [init_symbol final_to_stack_pda]) (q, [], []))" (is "?l \<longleftrightarrow> ?r")
 proof
-  assume "\<exists>q \<gamma>. q \<in> final_states M \<and> pda.steps M (init_state M, w, [init_symbol M]) (q, [], \<gamma>)"
+  assume ?l
   then obtain q \<gamma> where q_final: "q \<in> final_states M" and steps: "pda.steps M (init_state M, w, [init_symbol M]) (q, [], \<gamma>)" by blast
-  from steps have *: "pda.steps final_to_stack_pda (Old_st (init_state M), w, [Old_sym (init_symbol M), New_sym]) 
+  obtain Z \<alpha> where map_\<gamma>_def: "\<alpha>_with_new \<gamma> = Z#\<alpha>"
+    by (auto intro: list.exhaust_sel)
+  from q_final have "(New_final, [Z]) \<in> final_to_stack_eps_fun (Old_st q) Z"
+    by (induction "Old_st q" Z rule: final_to_stack_eps_fun.induct) auto
+
+  with map_\<gamma>_def have "pda.step\<^sub>1 final_to_stack_pda (Old_st q, [], \<alpha>_with_new \<gamma>) (New_final, [], Z#\<alpha>)"
+    using pda.step\<^sub>1_rule[OF pda_final_to_stack] by (simp add: final_to_stack_pda_def)
+
+  moreover from steps have "pda.steps final_to_stack_pda (Old_st (init_state M), w, [Old_sym (init_symbol M), New_sym]) 
                                                     (Old_st q, [], \<alpha>_with_new \<gamma>)"
     using final_to_stack_pda_steps by simp
-  have **: "pda.step\<^sub>1 final_to_stack_pda (init_state final_to_stack_pda, w, [init_symbol final_to_stack_pda])
+
+  moreover have "pda.step\<^sub>1 final_to_stack_pda (init_state final_to_stack_pda, w, [init_symbol final_to_stack_pda])
                                          (Old_st (init_state M), w, [Old_sym (init_symbol M), New_sym])"
     using pda.step\<^sub>1_rule[OF pda_final_to_stack] by (simp add: final_to_stack_pda_def)
-  obtain Z' \<alpha>' where map_\<gamma>_def: "\<alpha>_with_new \<gamma> = Z'#\<alpha>'"
-    by (auto intro: list.exhaust_sel)
-  from q_final have "(New_final, [Z']) \<in> final_to_stack_eps_fun (Old_st q) Z'"
-    by (induction "Old_st q" Z' rule: final_to_stack_eps_fun.induct) auto
-  with map_\<gamma>_def have ***: "pda.step\<^sub>1 final_to_stack_pda (Old_st q, [], \<alpha>_with_new \<gamma>) (New_final, [], Z'#\<alpha>')"
-    using pda.step\<^sub>1_rule[OF pda_final_to_stack] by (simp add: final_to_stack_pda_def)
-  have ****: "pda.steps final_to_stack_pda (New_final, [], Z'#\<alpha>') (New_final, [], [])"
+
+  moreover have "pda.steps final_to_stack_pda (New_final, [], Z#\<alpha>) (New_final, [], [])"
     using final_to_stack_pda_final_dump by simp
-  from * ** *** **** have "pda.steps final_to_stack_pda
-                              (init_state final_to_stack_pda, w, [init_symbol final_to_stack_pda]) (New_final, [], [])"
-    using pda.step\<^sub>1_stepn_one[OF pda_final_to_stack] pda.stepn_steps[OF pda_final_to_stack]
-          pda.steps_trans[OF pda_final_to_stack] by metis
-  thus "\<exists>q. pda.steps final_to_stack_pda (init_state final_to_stack_pda, w, [init_symbol final_to_stack_pda]) (q, [], [])" by blast
+
+  ultimately show ?r 
+    using pda.step\<^sub>1_steps[OF pda_final_to_stack] pda.steps_trans[OF pda_final_to_stack] by metis
 next
-  assume "\<exists>q. pda.steps final_to_stack_pda (init_state final_to_stack_pda, w, [init_symbol final_to_stack_pda]) (q, [], [])"
+  assume ?r
   then obtain q where steps: "pda.steps final_to_stack_pda (New_init, w, [New_sym]) (q, [], [])"
-    unfolding final_to_stack_pda_def by auto
+    by (auto simp: final_to_stack_pda_def)
   hence q_def: "q = New_final"
     using final_to_stack_pda_empty_only_final by simp
   with steps obtain n where stepn: "pda.stepn final_to_stack_pda n (New_init, w, [New_sym]) (New_final, [], [])"
     using pda.stepn_steps[OF pda_final_to_stack] by blast
   then obtain n' where "n = Suc (Suc n')"
-    using final_to_stack_pda_path_length by (metis Suc_le_D Suc_le_mono numeral_2_eq_2) 
+    using final_to_stack_pda_path_length by blast
   with stepn obtain p k \<alpha> where p_final: "p \<in> final_states M" and stepn': "pda.stepn final_to_stack_pda k 
                   (Old_st (init_state M), w, [Old_sym (init_symbol M), New_sym]) (Old_st p, [], \<alpha>)"
     using final_to_stack_pda_split_path by blast
@@ -486,7 +423,7 @@ next
     by (metis (no_types, opaque_lifting) append_Cons append_Nil list.simps(8,9))
   with stepn' have "pda.stepn M k (init_state M, w, [init_symbol M]) (p, [], \<alpha>')"
     using final_to_stack_pda_stepn by simp
-  with p_final show "\<exists>q \<gamma>. q \<in> final_states M \<and> pda.steps M (init_state M, w, [init_symbol M]) (q, [], \<gamma>)"
+  with p_final show ?l
     using stepn_steps by blast
 qed
 
