TaskinBA/Stack_To_Final_PDA.thy
@@ -43,99 +43,80 @@ proof (standard, goal_cases)
   have "finite (stack_to_final_trans_fun p x z)"
     by (induction p x z rule: stack_to_final_trans_fun.induct) (auto simp: finite_trans)
   then show ?case
-    unfolding stack_to_final_pda_def by simp
+    by (simp add: stack_to_final_pda_def)
 next
   case (2 p z)
   have "finite (stack_to_final_eps_fun p z)"
     by (induction p z rule: stack_to_final_eps_fun.induct) (auto simp: finite_eps)
   then show ?case
-    unfolding stack_to_final_pda_def by simp
+    by (simp add: stack_to_final_pda_def)
 qed
 
 lemma stack_to_final_pda_trans:
   "(p, \<beta>) \<in> trans_fun M q a Z \<longleftrightarrow> 
           (Old_st p, map Old_sym \<beta>) \<in> trans_fun stack_to_final_pda (Old_st q) a (Old_sym Z)"
-proof
-  assume "(p, \<beta>) \<in> trans_fun M q a Z"
-  thus "(Old_st p, map Old_sym \<beta>) \<in> trans_fun stack_to_final_pda (Old_st q) a (Old_sym Z)"
-    unfolding stack_to_final_pda_def by auto
-next
-  assume "(Old_st p, map Old_sym \<beta>) \<in> trans_fun stack_to_final_pda (Old_st q) a (Old_sym Z)"
-  hence "(Old_st p, map Old_sym \<beta>) \<in> (\<lambda>(p, \<alpha>). (Old_st p, map Old_sym \<alpha>)) ` (trans_fun M q a Z)"
-    unfolding stack_to_final_pda_def by simp
-  then obtain p' \<alpha>' where old_eq: "(Old_st p, map Old_sym \<beta>) = (Old_st p', map Old_sym \<alpha>')" and elem: "(p', \<alpha>') \<in> (trans_fun M q a Z)" by auto
-  from old_eq have p_eq: "p = p'" by simp
-  from old_eq have \<beta>_eq: "\<beta> = \<alpha>'"
-    by (metis list.inj_map_strong prod.inject sym_extended.inject)
-  from p_eq \<beta>_eq elem show "(p, \<beta>) \<in> trans_fun M q a Z" by simp
-qed
+  apply (rule iffI)
+   apply (auto simp: stack_to_final_pda_def)
+  apply (metis list.inj_map_strong sym_extended.inject)
+  done
 
 lemma stack_to_final_pda_eps:
   "(p, \<beta>) \<in> eps_fun M q Z \<longleftrightarrow> (Old_st p, map Old_sym \<beta>) \<in> eps_fun stack_to_final_pda (Old_st q) (Old_sym Z)"
-proof
-  assume "(p, \<beta>) \<in> eps_fun M q Z"
-  thus "(Old_st p, map Old_sym \<beta>) \<in> eps_fun stack_to_final_pda (Old_st q) (Old_sym Z)"
-    unfolding stack_to_final_pda_def by auto
-next
-  assume "(Old_st p, map Old_sym \<beta>) \<in> eps_fun stack_to_final_pda (Old_st q) (Old_sym Z)"
-  hence "(Old_st p, map Old_sym \<beta>) \<in> (\<lambda>(p, \<alpha>). (Old_st p, map Old_sym \<alpha>)) ` (eps_fun M q Z)"
-    unfolding stack_to_final_pda_def by simp
-  then obtain p' \<alpha>' where old_eq: "(Old_st p, map Old_sym \<beta>) = (Old_st p', map Old_sym \<alpha>')" and elem: "(p', \<alpha>') \<in> (eps_fun M q Z)" by auto
-  from old_eq have p_eq: "p = p'" by simp
-  from old_eq have \<beta>_eq: "\<beta> = \<alpha>'"
-    by (metis list.inj_map_strong prod.inject sym_extended.inject)
-  from p_eq \<beta>_eq elem show "(p, \<beta>) \<in> eps_fun M q Z" by simp
-qed
+  apply (rule iffI)
+   apply (auto simp: stack_to_final_pda_def)
+  apply (metis list.inj_map_strong sym_extended.inject)
+  done
 
 lemma stack_to_final_pda_step: 
   "pda.step\<^sub>1 M (p\<^sub>1, w\<^sub>1, \<alpha>\<^sub>1) (p\<^sub>2, w\<^sub>2, \<alpha>\<^sub>2) \<longleftrightarrow>
-      pda.step\<^sub>1 stack_to_final_pda (Old_st p\<^sub>1, w\<^sub>1, map Old_sym \<alpha>\<^sub>1) (Old_st p\<^sub>2, w\<^sub>2, map Old_sym \<alpha>\<^sub>2)"
+      pda.step\<^sub>1 stack_to_final_pda (Old_st p\<^sub>1, w\<^sub>1, map Old_sym \<alpha>\<^sub>1) (Old_st p\<^sub>2, w\<^sub>2, map Old_sym \<alpha>\<^sub>2)" (is "?l \<longleftrightarrow> ?r")
 proof
-  assume "pda.step\<^sub>1 M (p\<^sub>1, w\<^sub>1, \<alpha>\<^sub>1) (p\<^sub>2, w\<^sub>2, \<alpha>\<^sub>2)"
-  then obtain Z' \<alpha>' where \<alpha>\<^sub>1_def: "\<alpha>\<^sub>1 = Z' # \<alpha>'" and rule: "(\<exists>\<beta>. w\<^sub>2 = w\<^sub>1 \<and> \<alpha>\<^sub>2 = \<beta>@\<alpha>' \<and> (p\<^sub>2, \<beta>) \<in> eps_fun M p\<^sub>1 Z') 
-                            \<or> (\<exists>a \<beta>. w\<^sub>1 = a # w\<^sub>2 \<and> \<alpha>\<^sub>2 = \<beta>@\<alpha>' \<and> (p\<^sub>2,\<beta>) \<in> trans_fun M p\<^sub>1 a Z')"
+  assume ?l
+  then obtain Z \<alpha> where \<alpha>\<^sub>1_def: "\<alpha>\<^sub>1 = Z # \<alpha>" and rule: "(\<exists>\<beta>. w\<^sub>2 = w\<^sub>1 \<and> \<alpha>\<^sub>2 = \<beta>@\<alpha> \<and> (p\<^sub>2, \<beta>) \<in> eps_fun M p\<^sub>1 Z) 
+                            \<or> (\<exists>a \<beta>. w\<^sub>1 = a # w\<^sub>2 \<and> \<alpha>\<^sub>2 = \<beta>@\<alpha> \<and> (p\<^sub>2,\<beta>) \<in> trans_fun M p\<^sub>1 a Z)"
     using step\<^sub>1_rule_ext by auto
-  from rule have "(\<exists>\<beta>. w\<^sub>2 = w\<^sub>1 \<and> map Old_sym \<alpha>\<^sub>2 = map Old_sym \<beta> @ map Old_sym \<alpha>' \<and> (Old_st p\<^sub>2, map Old_sym \<beta>) \<in> eps_fun stack_to_final_pda (Old_st p\<^sub>1) (Old_sym Z')) 
-            \<or> (\<exists>a \<beta>. w\<^sub>1 = a # w\<^sub>2 \<and> map Old_sym \<alpha>\<^sub>2 = map Old_sym \<beta> @ map Old_sym \<alpha>' \<and> 
-                 (Old_st p\<^sub>2, map Old_sym \<beta>) \<in> trans_fun stack_to_final_pda (Old_st p\<^sub>1) a (Old_sym Z'))"
+  from rule have "(\<exists>\<beta>. w\<^sub>2 = w\<^sub>1 \<and> map Old_sym \<alpha>\<^sub>2 = map Old_sym \<beta> @ map Old_sym \<alpha> \<and> (Old_st p\<^sub>2, map Old_sym \<beta>) \<in> eps_fun stack_to_final_pda (Old_st p\<^sub>1) (Old_sym Z)) 
+            \<or> (\<exists>a \<beta>. w\<^sub>1 = a # w\<^sub>2 \<and> map Old_sym \<alpha>\<^sub>2 = map Old_sym \<beta> @ map Old_sym \<alpha> \<and> 
+                 (Old_st p\<^sub>2, map Old_sym \<beta>) \<in> trans_fun stack_to_final_pda (Old_st p\<^sub>1) a (Old_sym Z))"
     using stack_to_final_pda_trans stack_to_final_pda_eps by auto
-  hence "(\<exists>\<beta>. w\<^sub>2 = w\<^sub>1 \<and> map Old_sym \<alpha>\<^sub>2 = \<beta> @ map Old_sym \<alpha>' \<and> (Old_st p\<^sub>2, \<beta>) \<in> eps_fun stack_to_final_pda (Old_st p\<^sub>1) (Old_sym Z')) 
-            \<or> (\<exists>a \<beta>. w\<^sub>1 = a # w\<^sub>2 \<and> map Old_sym \<alpha>\<^sub>2 = \<beta> @ map Old_sym \<alpha>' \<and> (Old_st p\<^sub>2, \<beta>) \<in> trans_fun stack_to_final_pda (Old_st p\<^sub>1) a (Old_sym Z'))" 
+  hence "(\<exists>\<beta>. w\<^sub>2 = w\<^sub>1 \<and> map Old_sym \<alpha>\<^sub>2 = \<beta> @ map Old_sym \<alpha> \<and> (Old_st p\<^sub>2, \<beta>) \<in> eps_fun stack_to_final_pda (Old_st p\<^sub>1) (Old_sym Z)) 
+            \<or> (\<exists>a \<beta>. w\<^sub>1 = a # w\<^sub>2 \<and> map Old_sym \<alpha>\<^sub>2 = \<beta> @ map Old_sym \<alpha> \<and> (Old_st p\<^sub>2, \<beta>) \<in> trans_fun stack_to_final_pda (Old_st p\<^sub>1) a (Old_sym Z))" 
     by blast
-  with \<alpha>\<^sub>1_def show "pda.step\<^sub>1 stack_to_final_pda (Old_st p\<^sub>1, w\<^sub>1, map Old_sym \<alpha>\<^sub>1) (Old_st p\<^sub>2, w\<^sub>2, map Old_sym \<alpha>\<^sub>2)"
+  with \<alpha>\<^sub>1_def show ?r
     using pda.step\<^sub>1_rule[OF pda_stack_to_final] by simp
 next
-  assume "pda.step\<^sub>1 stack_to_final_pda (Old_st p\<^sub>1, w\<^sub>1, map Old_sym \<alpha>\<^sub>1) (Old_st p\<^sub>2, w\<^sub>2, map Old_sym \<alpha>\<^sub>2)"
-  then obtain Z' \<alpha>' where map_\<alpha>\<^sub>1_def: "map Old_sym \<alpha>\<^sub>1 = Old_sym Z' # map Old_sym \<alpha>'" and 
-     rule: "(\<exists>\<beta>. w\<^sub>2 = w\<^sub>1 \<and> map Old_sym \<alpha>\<^sub>2 = \<beta> @ map Old_sym \<alpha>' \<and> (Old_st p\<^sub>2, \<beta>) \<in> eps_fun stack_to_final_pda (Old_st p\<^sub>1) (Old_sym Z')) 
-         \<or> (\<exists>a \<beta>. w\<^sub>1 = a # w\<^sub>2 \<and> map Old_sym \<alpha>\<^sub>2 = \<beta>@ map Old_sym \<alpha>' \<and> (Old_st p\<^sub>2,\<beta>) \<in> trans_fun stack_to_final_pda (Old_st p\<^sub>1) a (Old_sym Z'))"
+  assume ?r
+  then obtain Z \<alpha> where map_\<alpha>\<^sub>1_def: "map Old_sym \<alpha>\<^sub>1 = Old_sym Z # map Old_sym \<alpha>" and 
+     rule: "(\<exists>\<beta>. w\<^sub>2 = w\<^sub>1 \<and> map Old_sym \<alpha>\<^sub>2 = \<beta> @ map Old_sym \<alpha> \<and> (Old_st p\<^sub>2, \<beta>) \<in> eps_fun stack_to_final_pda (Old_st p\<^sub>1) (Old_sym Z)) 
+         \<or> (\<exists>a \<beta>. w\<^sub>1 = a # w\<^sub>2 \<and> map Old_sym \<alpha>\<^sub>2 = \<beta>@ map Old_sym \<alpha> \<and> (Old_st p\<^sub>2,\<beta>) \<in> trans_fun stack_to_final_pda (Old_st p\<^sub>1) a (Old_sym Z))"
     using pda.step\<^sub>1_rule_ext[OF pda_stack_to_final] by auto
-  from map_\<alpha>\<^sub>1_def have \<alpha>\<^sub>1_def: "\<alpha>\<^sub>1 = Z' # \<alpha>'"
+  from map_\<alpha>\<^sub>1_def have \<alpha>\<^sub>1_def: "\<alpha>\<^sub>1 = Z # \<alpha>"
     by (metis list.inj_map_strong list.simps(9) sym_extended.inject)
-  from rule have "(\<exists>\<beta>. w\<^sub>2 = w\<^sub>1 \<and> map Old_sym \<alpha>\<^sub>2 = map Old_sym \<beta>@ map Old_sym \<alpha>' \<and> (Old_st p\<^sub>2, map Old_sym \<beta>) \<in> eps_fun stack_to_final_pda (Old_st p\<^sub>1) (Old_sym Z')) 
-     \<or> (\<exists>a \<beta>. w\<^sub>1 = a # w\<^sub>2 \<and> map Old_sym \<alpha>\<^sub>2 = map Old_sym \<beta>@ map Old_sym \<alpha>' \<and> (Old_st p\<^sub>2, map Old_sym \<beta>) \<in> trans_fun stack_to_final_pda (Old_st p\<^sub>1) a (Old_sym Z'))"
+  from rule have "(\<exists>\<beta>. w\<^sub>2 = w\<^sub>1 \<and> map Old_sym \<alpha>\<^sub>2 = map Old_sym \<beta>@ map Old_sym \<alpha> \<and> (Old_st p\<^sub>2, map Old_sym \<beta>) \<in> eps_fun stack_to_final_pda (Old_st p\<^sub>1) (Old_sym Z)) 
+     \<or> (\<exists>a \<beta>. w\<^sub>1 = a # w\<^sub>2 \<and> map Old_sym \<alpha>\<^sub>2 = map Old_sym \<beta>@ map Old_sym \<alpha> \<and> (Old_st p\<^sub>2, map Old_sym \<beta>) \<in> trans_fun stack_to_final_pda (Old_st p\<^sub>1) a (Old_sym Z))"
     using append_eq_map_conv[where ?f = Old_sym] by metis
-  hence "(\<exists>\<beta>. w\<^sub>2 = w\<^sub>1 \<and> \<alpha>\<^sub>2 = \<beta>@\<alpha>' \<and> (p\<^sub>2, \<beta>) \<in> eps_fun M p\<^sub>1 Z')
-    \<or> (\<exists>a \<beta>. w\<^sub>1 = a # w\<^sub>2 \<and> \<alpha>\<^sub>2 = \<beta>@\<alpha>' \<and> (p\<^sub>2,\<beta>) \<in> trans_fun M p\<^sub>1 a Z')"
+  hence "(\<exists>\<beta>. w\<^sub>2 = w\<^sub>1 \<and> \<alpha>\<^sub>2 = \<beta>@\<alpha> \<and> (p\<^sub>2, \<beta>) \<in> eps_fun M p\<^sub>1 Z)
+    \<or> (\<exists>a \<beta>. w\<^sub>1 = a # w\<^sub>2 \<and> \<alpha>\<^sub>2 = \<beta>@\<alpha> \<and> (p\<^sub>2,\<beta>) \<in> trans_fun M p\<^sub>1 a Z)"
     using stack_to_final_pda_trans stack_to_final_pda_eps by (metis list.inj_map_strong sym_extended.inject map_append)
-  with \<alpha>\<^sub>1_def show "pda.step\<^sub>1 M (p\<^sub>1, w\<^sub>1, \<alpha>\<^sub>1) (p\<^sub>2, w\<^sub>2, \<alpha>\<^sub>2)"
+  with \<alpha>\<^sub>1_def show ?l
     using step\<^sub>1_rule by simp
 qed
 
-abbreviation "\<alpha>_with_new \<alpha> \<equiv> map Old_sym \<alpha> @ [New_sym]"
+abbreviation \<alpha>_with_new :: "'s list \<Rightarrow> 's sym_extended list" where
+  "\<alpha>_with_new \<alpha> \<equiv> map Old_sym \<alpha> @ [New_sym]"
 
 lemma stack_to_final_pda_step\<^sub>1_drop:
   assumes "pda.step\<^sub>1 stack_to_final_pda (Old_st p\<^sub>1, w\<^sub>1, \<alpha>_with_new \<alpha>\<^sub>1) 
                                             (Old_st p\<^sub>2, w\<^sub>2, \<alpha>_with_new \<alpha>\<^sub>2)"
     shows "pda.step\<^sub>1 M (p\<^sub>1, w\<^sub>1, \<alpha>\<^sub>1) (p\<^sub>2, w\<^sub>2, \<alpha>\<^sub>2)"
 proof -
-  from assms obtain Z' \<alpha>' where map_\<alpha>\<^sub>1_def: "\<alpha>_with_new \<alpha>\<^sub>1 = Z' # \<alpha>'" and
-    rule: "(\<exists>\<beta>. w\<^sub>2 = w\<^sub>1 \<and> \<alpha>_with_new \<alpha>\<^sub>2 = \<beta>@\<alpha>' \<and> (Old_st p\<^sub>2, \<beta>) \<in> stack_to_final_eps_fun (Old_st p\<^sub>1) Z') 
-         \<or> (\<exists>a \<beta>. w\<^sub>1 = a # w\<^sub>2 \<and> \<alpha>_with_new \<alpha>\<^sub>2 = \<beta>@\<alpha>' \<and> (Old_st p\<^sub>2,\<beta>) \<in> stack_to_final_trans_fun (Old_st p\<^sub>1) a Z')"
+  from assms obtain Z \<alpha> where \<alpha>\<^sub>1_with_new_def: "\<alpha>_with_new \<alpha>\<^sub>1 = Z # \<alpha>" and
+    rule: "(\<exists>\<beta>. w\<^sub>2 = w\<^sub>1 \<and> \<alpha>_with_new \<alpha>\<^sub>2 = \<beta>@\<alpha> \<and> (Old_st p\<^sub>2, \<beta>) \<in> stack_to_final_eps_fun (Old_st p\<^sub>1) Z) 
+         \<or> (\<exists>a \<beta>. w\<^sub>1 = a # w\<^sub>2 \<and> \<alpha>_with_new \<alpha>\<^sub>2 = \<beta>@\<alpha> \<and> (Old_st p\<^sub>2,\<beta>) \<in> stack_to_final_trans_fun (Old_st p\<^sub>1) a Z)"
     using pda.step\<^sub>1_rule_ext[OF pda_stack_to_final] by (auto simp: stack_to_final_pda_def)
-  from rule have "Z' \<noteq> New_sym"
-    by (induction "Old_st p\<^sub>1" Z' rule: stack_to_final_eps_fun.induct) auto
-  with map_\<alpha>\<^sub>1_def have "map Old_sym \<alpha>\<^sub>1 \<noteq> []" by auto
+  from rule have "Z \<noteq> New_sym"
+    by (induction "Old_st p\<^sub>1" Z rule: stack_to_final_eps_fun.induct) auto
+  with \<alpha>\<^sub>1_with_new_def have "map Old_sym \<alpha>\<^sub>1 \<noteq> []" by auto
   with assms have "pda.step\<^sub>1 stack_to_final_pda (Old_st p\<^sub>1, w\<^sub>1, map Old_sym \<alpha>\<^sub>1) 
                                                 (Old_st p\<^sub>2, w\<^sub>2, map Old_sym \<alpha>\<^sub>2)"
     using pda.step\<^sub>1_stack_drop[OF pda_stack_to_final] by blast
@@ -147,47 +128,26 @@ lemma stack_to_final_pda_from_old:
   assumes "pda.step\<^sub>1 stack_to_final_pda (Old_st p\<^sub>1, w\<^sub>1, \<alpha>\<^sub>1) (p\<^sub>2, w\<^sub>2, \<alpha>\<^sub>2)"
     shows "(\<exists>p\<^sub>2'. p\<^sub>2 = Old_st p\<^sub>2') \<or> p\<^sub>2 = New_final"
 proof -
-  from assms obtain Z' \<alpha>' where "\<alpha>\<^sub>1 = Z'#\<alpha>'" and 
-            rule: "(\<exists>\<beta>. w\<^sub>2 = w\<^sub>1 \<and> \<alpha>\<^sub>2 = \<beta>@\<alpha>' \<and> (p\<^sub>2, \<beta>) \<in> stack_to_final_eps_fun (Old_st p\<^sub>1) Z') 
-                      \<or> (\<exists>a \<beta>. w\<^sub>1 = a # w\<^sub>2 \<and> \<alpha>\<^sub>2 = \<beta>@\<alpha>' \<and> (p\<^sub>2,\<beta>) \<in> stack_to_final_trans_fun (Old_st p\<^sub>1) a Z')"
-    using pda.step\<^sub>1_rule_ext[OF pda_stack_to_final] by (auto simp: stack_to_final_pda_def)
-  from rule show ?thesis by (induction "Old_st p\<^sub>1" Z' rule: stack_to_final_eps_fun.induct) auto
+  from assms obtain Z \<alpha> where 
+            "(\<exists>\<beta>. w\<^sub>2 = w\<^sub>1 \<and> \<alpha>\<^sub>2 = \<beta>@\<alpha> \<and> (p\<^sub>2, \<beta>) \<in> stack_to_final_eps_fun (Old_st p\<^sub>1) Z) 
+              \<or> (\<exists>a \<beta>. w\<^sub>1 = a # w\<^sub>2 \<and> \<alpha>\<^sub>2 = \<beta>@\<alpha> \<and> (p\<^sub>2,\<beta>) \<in> stack_to_final_trans_fun (Old_st p\<^sub>1) a Z)"
+    using pda.step\<^sub>1_rule_ext[OF pda_stack_to_final] by (auto simp: stack_to_final_pda_def)+
+  thus ?thesis 
+    by (induction "Old_st p\<^sub>1" Z rule: stack_to_final_eps_fun.induct) auto
 qed
 
 lemma stack_to_final_pda_no_step_final:
   "\<not>pda.step\<^sub>1 stack_to_final_pda (New_final, w\<^sub>1, \<alpha>\<^sub>1) (p, w\<^sub>2, \<alpha>\<^sub>2)"
-proof (cases \<alpha>\<^sub>1)
-  case Nil
-  thus ?thesis
-    using pda.step\<^sub>1_empty_stack[OF pda_stack_to_final] by simp
-next
-  case (Cons Z' \<alpha>')
-  have "(\<nexists>\<beta>. (p, \<beta>) \<in> stack_to_final_eps_fun New_final Z') 
-                         \<or> (\<nexists>a \<beta>. (p,\<beta>) \<in> stack_to_final_trans_fun New_final a Z')"
-    by simp
-  with Cons show ?thesis
-    using pda.step\<^sub>1_rule[OF pda_stack_to_final] by (simp add: stack_to_final_pda_def)
-qed
+  apply (cases \<alpha>\<^sub>1)
+   apply (simp add: pda.step\<^sub>1_empty_stack[OF pda_stack_to_final])
+  apply (use pda.step\<^sub>1_rule[OF pda_stack_to_final] stack_to_final_pda_def in simp)
+  done
 
 lemma stack_to_final_pda_from_oldn:
   assumes "pda.steps stack_to_final_pda (Old_st p\<^sub>1, w\<^sub>1, \<alpha>\<^sub>1) (p\<^sub>2, w\<^sub>2, \<alpha>\<^sub>2)"
   shows "\<exists>q'. p\<^sub>2 = Old_st q' \<or> p\<^sub>2 = New_final"
-using assms proof (induction "(Old_st p\<^sub>1, w\<^sub>1, \<alpha>\<^sub>1)" "(p\<^sub>2, w\<^sub>2, \<alpha>\<^sub>2)" arbitrary: p\<^sub>1 w\<^sub>1 \<alpha>\<^sub>1 rule: pda.steps_induct[OF pda_stack_to_final])
-  case (3 w\<^sub>1 \<alpha>\<^sub>1 p' w' \<alpha>')
-  from 3(1) have case_dist: "(\<exists>p''. p' = Old_st p'') \<or> p' = New_final"
-    using stack_to_final_pda_from_old by simp
-  then show ?case proof (cases)
-    assume "\<exists>p''. p' = Old_st p''"
-    then obtain p'' where "p' = Old_st p''" by blast
-    with 3(2,3) show ?thesis by blast
-  next
-    assume "\<not>(\<exists>p''. p' = Old_st p'')"
-    with case_dist have "p' = New_final" by simp
-    with 3(2) show ?thesis
-      using pda.steps_not_refl_split_first[OF pda_stack_to_final]
-            stack_to_final_pda_no_step_final by blast
-  qed
-qed (blast intro: assms)+
+by (induction "(Old_st p\<^sub>1, w\<^sub>1, \<alpha>\<^sub>1)" "(p\<^sub>2, w\<^sub>2, \<alpha>\<^sub>2)" arbitrary: p\<^sub>2 w\<^sub>2 \<alpha>\<^sub>2 rule: pda.steps_induct2[OF pda_stack_to_final])
+  (use assms stack_to_final_pda_from_old stack_to_final_pda_no_step_final in blast)+
 
 lemma stack_to_final_pda_to_old:
   assumes "pda.step\<^sub>1 stack_to_final_pda (p\<^sub>1, w\<^sub>1, \<alpha>\<^sub>1) (Old_st p\<^sub>2, w\<^sub>2, \<alpha>\<^sub>2)"
@@ -198,43 +158,30 @@ lemma stack_to_final_pda_bottom_elem:
   assumes "pda.steps stack_to_final_pda (Old_st p\<^sub>1, w\<^sub>1, \<alpha>_with_new \<alpha>\<^sub>1)
                                          (Old_st p\<^sub>2, w\<^sub>2, \<gamma>)"
   shows "\<exists>\<alpha>. \<gamma> = \<alpha>_with_new \<alpha>"
-proof -
-  from assms obtain n where stepn: "pda.stepn stack_to_final_pda n (Old_st p\<^sub>1, w\<^sub>1, \<alpha>_with_new \<alpha>\<^sub>1)
-                                                                   (Old_st p\<^sub>2, w\<^sub>2, \<gamma>)"
-    using pda.stepn_steps[OF pda_stack_to_final] by blast
-  thus ?thesis proof 
-   (induction n "(Old_st p\<^sub>1, w\<^sub>1, \<alpha>_with_new \<alpha>\<^sub>1)" "(Old_st p\<^sub>2, w\<^sub>2, \<gamma>)"
-       arbitrary: p\<^sub>2 w\<^sub>2 \<gamma> rule: pda.stepn.induct[OF pda_stack_to_final])
-    case (3 n p\<^sub>2 w\<^sub>2 \<alpha>\<^sub>2 w\<^sub>3 \<alpha>\<^sub>3 p\<^sub>3)
-    from 3(1) have steps: "pda.steps stack_to_final_pda (Old_st p\<^sub>1, w\<^sub>1, \<alpha>_with_new \<alpha>\<^sub>1) (p\<^sub>2, w\<^sub>2, \<alpha>\<^sub>2)"
-      using pda.stepn_steps[OF pda_stack_to_final] by blast
-    obtain p\<^sub>2' where p\<^sub>2_def: "p\<^sub>2 = Old_st p\<^sub>2'"
-      using stack_to_final_pda_from_oldn[OF steps] stack_to_final_pda_to_old[OF 3(3)] by blast
-    with 3(1,2) have \<alpha>\<^sub>2_def: "\<exists>\<alpha>. \<alpha>\<^sub>2 = \<alpha>_with_new \<alpha>" by simp
-    from p\<^sub>2_def 3(3) obtain Z' \<alpha>' where \<alpha>\<^sub>2_split: "\<alpha>\<^sub>2 = Z' # \<alpha>'" and rule:
-    "(\<exists>\<beta>. w\<^sub>3 = w\<^sub>2 \<and> \<alpha>\<^sub>3 = \<beta> @ \<alpha>' \<and> (Old_st p\<^sub>3, \<beta>) \<in> stack_to_final_eps_fun (Old_st p\<^sub>2') Z') 
-     \<or> (\<exists>a \<beta>. w\<^sub>2 = a # w\<^sub>3 \<and> \<alpha>\<^sub>3 = \<beta> @ \<alpha>' \<and> (Old_st p\<^sub>3, \<beta>) \<in> stack_to_final_trans_fun (Old_st p\<^sub>2') a Z')"
+using assms proof (induction "(Old_st p\<^sub>1, w\<^sub>1, \<alpha>_with_new \<alpha>\<^sub>1)" "(Old_st p\<^sub>2, w\<^sub>2, \<gamma>)" arbitrary: p\<^sub>2 w\<^sub>2 \<gamma>
+                          rule: pda.steps_induct2[OF pda_stack_to_final])
+  case (3 p\<^sub>2 w\<^sub>2 \<alpha>\<^sub>2 w\<^sub>3 \<alpha>\<^sub>3 p\<^sub>3)
+  obtain p\<^sub>2' where p\<^sub>2_def: "p\<^sub>2 = Old_st p\<^sub>2'"
+    using stack_to_final_pda_from_oldn[OF 3(1)] stack_to_final_pda_to_old[OF 3(2)] by blast
+  with 3(1,3) have \<alpha>\<^sub>2_def: "\<exists>\<alpha>. \<alpha>\<^sub>2 = \<alpha>_with_new \<alpha>" by simp
+  from 3(2)[unfolded p\<^sub>2_def] obtain Z \<alpha> where \<alpha>\<^sub>2_split: "\<alpha>\<^sub>2 = Z # \<alpha>" and rule:
+    "(\<exists>\<beta>. w\<^sub>3 = w\<^sub>2 \<and> \<alpha>\<^sub>3 = \<beta> @ \<alpha> \<and> (Old_st p\<^sub>3, \<beta>) \<in> stack_to_final_eps_fun (Old_st p\<^sub>2') Z) 
+     \<or> (\<exists>a \<beta>. w\<^sub>2 = a # w\<^sub>3 \<and> \<alpha>\<^sub>3 = \<beta> @ \<alpha> \<and> (Old_st p\<^sub>3, \<beta>) \<in> stack_to_final_trans_fun (Old_st p\<^sub>2') a Z)"
       using pda.step\<^sub>1_rule_ext[OF pda_stack_to_final] by (auto simp: stack_to_final_pda_def)
-    hence "\<exists>Z. Z' = Old_sym Z"
-      by (induction "Old_st p\<^sub>2'" Z' rule: stack_to_final_eps_fun.induct) auto
-    with \<alpha>\<^sub>2_def \<alpha>\<^sub>2_split have "\<exists>\<gamma>. \<alpha>' = \<alpha>_with_new \<gamma>"
+    from rule have "\<exists>Z'. Z = Old_sym Z'"
+      by (induction "Old_st p\<^sub>2'" Z rule: stack_to_final_eps_fun.induct) auto
+    with \<alpha>\<^sub>2_def \<alpha>\<^sub>2_split have "\<exists>\<gamma>. \<alpha> = \<alpha>_with_new \<gamma>"
       by (metis hd_append list.sel(1,3) map_tl sym_extended.simps(3) tl_append_if)
     with rule show ?case
-      by (induction "Old_st p\<^sub>2'" Z' rule: stack_to_final_eps_fun.induct, auto) (metis map_append)+
-  qed (auto simp: stepn)
-qed
+      by (induction "Old_st p\<^sub>2'" Z rule: stack_to_final_eps_fun.induct, auto) (metis map_append)+
+qed (rule assms, blast)
 
 lemma stack_to_final_pda_stepn:
   "pda.stepn M n (p\<^sub>1, w\<^sub>1, \<alpha>\<^sub>1) (p\<^sub>2, w\<^sub>2, \<alpha>\<^sub>2) \<longleftrightarrow> 
-            pda.stepn stack_to_final_pda n (Old_st p\<^sub>1, w\<^sub>1, \<alpha>_with_new \<alpha>\<^sub>1) (Old_st p\<^sub>2, w\<^sub>2, \<alpha>_with_new \<alpha>\<^sub>2)"
+            pda.stepn stack_to_final_pda n (Old_st p\<^sub>1, w\<^sub>1, \<alpha>_with_new \<alpha>\<^sub>1) (Old_st p\<^sub>2, w\<^sub>2, \<alpha>_with_new \<alpha>\<^sub>2)" (is "?l \<longleftrightarrow> ?r")
 proof
-  assume asm: "pda.stepn M n (p\<^sub>1, w\<^sub>1, \<alpha>\<^sub>1) (p\<^sub>2, w\<^sub>2, \<alpha>\<^sub>2)"
-  thus "pda.stepn stack_to_final_pda n (Old_st p\<^sub>1, w\<^sub>1, \<alpha>_with_new \<alpha>\<^sub>1) (Old_st p\<^sub>2, w\<^sub>2, \<alpha>_with_new \<alpha>\<^sub>2)"
+  show "?l \<Longrightarrow> ?r"
   proof (induction n "(p\<^sub>1, w\<^sub>1, \<alpha>\<^sub>1)" "(p\<^sub>2, w\<^sub>2, \<alpha>\<^sub>2)" arbitrary: p\<^sub>2 w\<^sub>2 \<alpha>\<^sub>2 rule: stepn.induct)
-    case refl\<^sub>n
-    then show ?case
-      by (simp add: pda.refl\<^sub>n[OF pda_stack_to_final])
-  next
     case (step\<^sub>n n p\<^sub>2 w\<^sub>2 \<alpha>\<^sub>2 p\<^sub>3 w\<^sub>3 \<alpha>\<^sub>3)
     from step\<^sub>n(3) have "pda.step\<^sub>1 stack_to_final_pda (Old_st p\<^sub>2, w\<^sub>2, map Old_sym \<alpha>\<^sub>2) (Old_st p\<^sub>3, w\<^sub>3, map Old_sym \<alpha>\<^sub>3)"
       using stack_to_final_pda_step by simp
@@ -242,56 +189,48 @@ proof
       using pda.step\<^sub>1_stack_app[OF pda_stack_to_final] by simp
     with step\<^sub>n(2) show ?case
       by (simp add: pda.step\<^sub>n[OF pda_stack_to_final])
-  qed
+  qed (simp add: pda.refl\<^sub>n[OF pda_stack_to_final])
 next
-  assume asm: "pda.stepn stack_to_final_pda n (Old_st p\<^sub>1, w\<^sub>1, \<alpha>_with_new \<alpha>\<^sub>1) (Old_st p\<^sub>2, w\<^sub>2, \<alpha>_with_new \<alpha>\<^sub>2)"
-  thus "pda.stepn M n (p\<^sub>1, w\<^sub>1, \<alpha>\<^sub>1) (p\<^sub>2, w\<^sub>2, \<alpha>\<^sub>2)"
+  assume r: ?r thus ?l
   proof (induction n "(Old_st p\<^sub>1, w\<^sub>1, \<alpha>_with_new \<alpha>\<^sub>1)" "(Old_st p\<^sub>2, w\<^sub>2, \<alpha>_with_new \<alpha>\<^sub>2)" 
                  arbitrary: p\<^sub>2 w\<^sub>2 \<alpha>\<^sub>2 rule: pda.stepn.induct[OF pda_stack_to_final])
-    case 2
-    from 2(1) have "\<alpha>\<^sub>1 = \<alpha>\<^sub>2"
-      by (metis list.inj_map_strong sym_extended.inject)
-    thus ?case by simp
-  next
     case (3 n p\<^sub>2 w\<^sub>2 \<alpha>\<^sub>2 w\<^sub>3 p\<^sub>3 \<alpha>\<^sub>3)
-    from 3(1) have steps: "pda.steps stack_to_final_pda (Old_st p\<^sub>1, w\<^sub>1, \<alpha>_with_new \<alpha>\<^sub>1) (p\<^sub>2, w\<^sub>2, \<alpha>\<^sub>2)"
+    from 3(1) have steps_3_1: "pda.steps stack_to_final_pda (Old_st p\<^sub>1, w\<^sub>1, \<alpha>_with_new \<alpha>\<^sub>1) (p\<^sub>2, w\<^sub>2, \<alpha>\<^sub>2)"
       using pda.stepn_steps[OF pda_stack_to_final] by blast
     obtain p\<^sub>2' where p\<^sub>2_def: "p\<^sub>2 = Old_st p\<^sub>2'"
-      using stack_to_final_pda_from_oldn[OF steps] stack_to_final_pda_to_old[OF 3(3)] by blast
-    with steps obtain \<gamma> where \<alpha>\<^sub>2_def: "\<alpha>\<^sub>2 = map Old_sym \<gamma> @ [New_sym]"
+      using stack_to_final_pda_from_oldn[OF steps_3_1] stack_to_final_pda_to_old[OF 3(3)] by blast
+    with steps_3_1 obtain \<gamma> where \<alpha>\<^sub>2_def: "\<alpha>\<^sub>2 = map Old_sym \<gamma> @ [New_sym]"
       using stack_to_final_pda_bottom_elem by blast
-    with p\<^sub>2_def 3(1,2) have *: "pda.stepn M n (p\<^sub>1, w\<^sub>1, \<alpha>\<^sub>1) (p\<^sub>2', w\<^sub>2, \<gamma>)" by simp
-    from p\<^sub>2_def \<alpha>\<^sub>2_def 3(3) have **: "pda.step\<^sub>1 M (p\<^sub>2', w\<^sub>2, \<gamma>) (p\<^sub>3, w\<^sub>3, \<alpha>\<^sub>3)"
+
+    with p\<^sub>2_def 3(1,2) have "pda.stepn M n (p\<^sub>1, w\<^sub>1, \<alpha>\<^sub>1) (p\<^sub>2', w\<^sub>2, \<gamma>)" by simp
+
+    moreover from p\<^sub>2_def \<alpha>\<^sub>2_def 3(3) have "pda.step\<^sub>1 M (p\<^sub>2', w\<^sub>2, \<gamma>) (p\<^sub>3, w\<^sub>3, \<alpha>\<^sub>3)"
       using stack_to_final_pda_step\<^sub>1_drop by simp
-    from * ** show ?case by simp
-  qed (simp add: asm)
+
+    ultimately show ?case by simp
+  qed (rule r, metis refl\<^sub>n list.inj_map_strong sym_extended.inject)
 qed
 
 lemma stack_to_final_pda_steps:
   "pda.steps M (p\<^sub>1, w\<^sub>1, \<alpha>\<^sub>1) (p\<^sub>2, w\<^sub>2, \<alpha>\<^sub>2) \<longleftrightarrow> 
             pda.steps stack_to_final_pda (Old_st p\<^sub>1, w\<^sub>1, \<alpha>_with_new \<alpha>\<^sub>1) (Old_st p\<^sub>2, w\<^sub>2, \<alpha>_with_new \<alpha>\<^sub>2)"
-  using stack_to_final_pda_stepn pda.stepn_steps[OF pda_stack_to_final] stepn_steps by simp
+using stack_to_final_pda_stepn pda.stepn_steps[OF pda_stack_to_final] stepn_steps by simp
 
 lemma stack_to_final_pda_first_step:
   assumes "pda.step\<^sub>1 stack_to_final_pda (New_init, w\<^sub>1, [New_sym]) (p\<^sub>2, w\<^sub>2, \<alpha>)"
   shows "p\<^sub>2 = Old_st (init_state M) \<and> w\<^sub>2 = w\<^sub>1 \<and> \<alpha> = [Old_sym (init_symbol M), New_sym]"
-proof -
-  from assms have "(\<exists>\<beta>. w\<^sub>2 = w\<^sub>1 \<and> \<alpha> = \<beta> \<and> (p\<^sub>2, \<beta>) \<in> stack_to_final_eps_fun New_init New_sym) 
-                   \<or> (\<exists>a \<beta>. w\<^sub>1 = a # w\<^sub>2 \<and> \<alpha> = \<beta> \<and> (p\<^sub>2, \<beta>) \<in> stack_to_final_trans_fun New_init a New_sym)"
-    using pda.step\<^sub>1_rule[OF pda_stack_to_final] by (simp add: stack_to_final_pda_def)
-  thus ?thesis by simp
-qed
+using assms pda.step\<^sub>1_rule[OF pda_stack_to_final] by (simp add: stack_to_final_pda_def)
 
 lemma stack_to_final_pda_last_step:
   assumes "pda.step\<^sub>1 stack_to_final_pda (p\<^sub>1, w\<^sub>1, \<alpha>\<^sub>1) (New_final, w\<^sub>2, \<alpha>\<^sub>2)"
     shows "\<exists>q. p\<^sub>1 = Old_st q \<and> w\<^sub>1 = w\<^sub>2 \<and> \<alpha>\<^sub>1 = New_sym # \<alpha>\<^sub>2"
 proof -
-  from assms obtain Z' \<alpha>' where \<alpha>\<^sub>1_def: "\<alpha>\<^sub>1 = Z' # \<alpha>'" and rule: 
-        "(\<exists>\<beta>. w\<^sub>2 = w\<^sub>1 \<and> \<alpha>\<^sub>2 = \<beta> @ \<alpha>' \<and> (New_final, \<beta>) \<in> stack_to_final_eps_fun p\<^sub>1 Z') 
-            \<or> (\<exists>a \<beta>. w\<^sub>1 = a # w\<^sub>2 \<and> \<alpha>\<^sub>2 = \<beta> @ \<alpha>' \<and> (New_final, \<beta>) \<in> stack_to_final_trans_fun p\<^sub>1 a Z')"
+  from assms obtain Z \<alpha> where \<alpha>\<^sub>1_def: "\<alpha>\<^sub>1 = Z # \<alpha>" and rule: 
+        "(\<exists>\<beta>. w\<^sub>2 = w\<^sub>1 \<and> \<alpha>\<^sub>2 = \<beta> @ \<alpha> \<and> (New_final, \<beta>) \<in> stack_to_final_eps_fun p\<^sub>1 Z) 
+            \<or> (\<exists>a \<beta>. w\<^sub>1 = a # w\<^sub>2 \<and> \<alpha>\<^sub>2 = \<beta> @ \<alpha> \<and> (New_final, \<beta>) \<in> stack_to_final_trans_fun p\<^sub>1 a Z)"
     using pda.step\<^sub>1_rule_ext[OF pda_stack_to_final] by (auto simp: stack_to_final_pda_def)
-  from rule have w_eq: "w\<^sub>2 = w\<^sub>1" and \<alpha>_eq: "\<alpha>\<^sub>2 = \<alpha>'" and elem: "\<exists>q. p\<^sub>1 = Old_st q \<and> Z' = New_sym"
-    by (induction p\<^sub>1 Z' rule: stack_to_final_eps_fun.induct) auto
+  from rule have "w\<^sub>2 = w\<^sub>1" and "\<alpha>\<^sub>2 = \<alpha>" and "\<exists>q. p\<^sub>1 = Old_st q \<and> Z = New_sym"
+    by (induction p\<^sub>1 Z rule: stack_to_final_eps_fun.induct) auto
   with \<alpha>\<^sub>1_def show ?thesis by simp
 qed
 
@@ -315,12 +254,8 @@ proof -
                               (Old_st (init_state M), w\<^sub>1, [Old_sym (init_symbol M), New_sym])
                               (Old_st q, w\<^sub>2, New_sym # \<gamma>)"
     using pda.stepn_split_last[OF pda_stack_to_final] stack_to_final_pda_last_step by blast
-  from stepn' have steps': "pda.steps stack_to_final_pda 
-                              (Old_st (init_state M), w\<^sub>1, [Old_sym (init_symbol M), New_sym])
-                              (Old_st q, w\<^sub>2, New_sym # \<gamma>)"
-    using pda.stepn_steps[OF pda_stack_to_final] by blast
-  from steps' have "\<exists>\<alpha>. New_sym # \<gamma> = \<alpha>_with_new \<alpha>"
-    using stack_to_final_pda_bottom_elem
+  from stepn' have "\<exists>\<alpha>. New_sym # \<gamma> = \<alpha>_with_new \<alpha>"
+    using stack_to_final_pda_bottom_elem pda.stepn_steps[OF pda_stack_to_final]
     by (metis (no_types, opaque_lifting) Cons_eq_appendI append_Nil list.map_disc_iff list.simps(9))
   hence "\<gamma> = []"
     by (metis Nil_is_map_conv hd_append2 hd_map list.sel(1,3) sym_extended.simps(3) tl_append_if)
@@ -329,66 +264,64 @@ qed
 
 lemma stack_to_final_pda_path_length:
   assumes "pda.stepn stack_to_final_pda n (New_init, w\<^sub>1, [New_sym]) (New_final, w\<^sub>2, \<gamma>)"
-    shows "n > 2"
+  shows "\<exists>n'. n = Suc (Suc (Suc n'))"
 proof -
-  from assms obtain n' where n_def: "n = Suc n'"
-    using pda.stepn_not_refl[OF pda_stack_to_final] gr0_implies_Suc by blast
-  with assms have fstep: "pda.step\<^sub>1 stack_to_final_pda (New_init, w\<^sub>1, [New_sym]) 
-                        (Old_st (init_state M), w\<^sub>1, [Old_sym (init_symbol M), New_sym])"
-                 and stepn: "pda.stepn stack_to_final_pda n' 
-                         (Old_st (init_state M), w\<^sub>1, [Old_sym (init_symbol M), New_sym])
-                         (New_final, w\<^sub>2, \<gamma>)"
-    using pda.stepn_split_first[OF pda_stack_to_final] stack_to_final_pda_first_step by blast+
+  from assms obtain n' where n_def: "n = Suc n'" and fstep: "pda.step\<^sub>1 stack_to_final_pda (New_init, w\<^sub>1, [New_sym]) 
+                                                          (Old_st (init_state M), w\<^sub>1, [Old_sym (init_symbol M), New_sym])"
+                                                  and stepn: "pda.stepn stack_to_final_pda n' 
+                                                          (Old_st (init_state M), w\<^sub>1, [Old_sym (init_symbol M), New_sym])
+                                                              (New_final, w\<^sub>2, \<gamma>)"
+    using pda.stepn_not_refl_split_first[OF pda_stack_to_final] stack_to_final_pda_first_step by blast
   from stepn obtain n'' where n'_def: "n' = Suc n''"
-    using pda.stepn_not_refl[OF pda_stack_to_final] gr0_implies_Suc by blast
+    using pda.stepn_not_refl_split_last[OF pda_stack_to_final] by blast
   with n_def assms have "\<exists>q. pda.stepn stack_to_final_pda n'' 
                               (Old_st (init_state M), w\<^sub>1, [Old_sym (init_symbol M), New_sym]) (Old_st q, w\<^sub>2, [New_sym])"
     using stack_to_final_pda_split_path by blast
   then obtain n''' where "n'' = Suc n'''"
-    using pda.stepn_not_refl[OF pda_stack_to_final] gr0_implies_Suc by blast
+    using pda.stepn_not_refl_split_last[OF pda_stack_to_final] by blast
   with n_def n'_def show ?thesis by simp
 qed
 
 lemma accepted_stack_to_final:  
 "(\<exists>q. pda.steps M (init_state M, w, [init_symbol M]) (q, [], [])) \<longleftrightarrow> (\<exists>q \<gamma>. q \<in> final_states stack_to_final_pda \<and> 
-  pda.steps stack_to_final_pda (init_state stack_to_final_pda, w, [init_symbol stack_to_final_pda]) (q, [], \<gamma>))"
+  pda.steps stack_to_final_pda (init_state stack_to_final_pda, w, [init_symbol stack_to_final_pda]) (q, [], \<gamma>))" (is "?l \<longleftrightarrow> ?r")
 proof
-  assume "\<exists>q. pda.steps M (init_state M, w, [init_symbol M]) (q, [], [])"
+  assume ?l
   then obtain q where "pda.steps M (init_state M, w, [init_symbol M]) (q, [], [])" by blast
-  hence *: "pda.steps stack_to_final_pda (Old_st (init_state M), w, [Old_sym (init_symbol M), New_sym]) (Old_st q, [], [New_sym])"
+  hence "pda.steps stack_to_final_pda (Old_st (init_state M), w, [Old_sym (init_symbol M), New_sym]) (Old_st q, [], [New_sym])"
     using stack_to_final_pda_steps by simp
-  have **: "pda.step\<^sub>1 stack_to_final_pda (init_state stack_to_final_pda, w, [init_symbol stack_to_final_pda]) 
+
+  moreover have "pda.step\<^sub>1 stack_to_final_pda (init_state stack_to_final_pda, w, [init_symbol stack_to_final_pda]) 
                                          (Old_st (init_state M), w, [Old_sym (init_symbol M), New_sym])"
     using pda.step\<^sub>1_rule[OF pda_stack_to_final] by (simp add: stack_to_final_pda_def)
-  have ***: "pda.step\<^sub>1 stack_to_final_pda (Old_st q, [], [New_sym]) (New_final, [], [])"
+
+  moreover have "pda.step\<^sub>1 stack_to_final_pda (Old_st q, [], [New_sym]) (New_final, [], [])"
     using pda.step\<^sub>1_rule[OF pda_stack_to_final] by (simp add: stack_to_final_pda_def)
-  from * ** *** have a1:
+
+  ultimately have a1:
     "pda.steps stack_to_final_pda (init_state stack_to_final_pda, w, [init_symbol stack_to_final_pda ]) (New_final, [], [])"
-    using pda.step\<^sub>1_stepn_one[OF pda_stack_to_final] pda.stepn_steps[OF pda_stack_to_final]
-          pda.steps_trans[OF pda_stack_to_final] by metis
-  have a2: "New_final \<in> final_states stack_to_final_pda"
+    using pda.step\<^sub>1_steps[OF pda_stack_to_final] pda.steps_trans[OF pda_stack_to_final] by metis
+
+  moreover have "New_final \<in> final_states stack_to_final_pda"
     by (simp add: stack_to_final_pda_def)
-  from a1 a2 show "\<exists>q \<gamma>. q \<in> final_states stack_to_final_pda \<and>
-                    pda.steps stack_to_final_pda (init_state stack_to_final_pda, w, [init_symbol stack_to_final_pda]) (q, [], \<gamma>)" by blast
+
+  ultimately show ?r by blast
 next
-  assume "\<exists>q \<gamma>. q \<in> final_states stack_to_final_pda \<and>
-          pda.steps stack_to_final_pda (init_state stack_to_final_pda, w, [init_symbol stack_to_final_pda]) (q, [], \<gamma>)"
+  assume ?r
   then obtain q \<gamma> where q_final: "q \<in> final_states stack_to_final_pda" and
-                "pda.steps stack_to_final_pda (init_state stack_to_final_pda, w, [init_symbol stack_to_final_pda]) (q, [], \<gamma>)" by blast
-  hence steps: "pda.steps stack_to_final_pda (New_init, w, [New_sym]) (q, [], \<gamma>)"
-    by (simp add: stack_to_final_pda_def)
+                steps: "pda.steps stack_to_final_pda (init_state stack_to_final_pda, w, [init_symbol stack_to_final_pda]) (q, [], \<gamma>)" by blast
   from q_final have q_def: "q = New_final"
     by (simp add: stack_to_final_pda_def)
   with steps obtain n where stepn: "pda.stepn stack_to_final_pda n (New_init, w, [New_sym]) (New_final, [], \<gamma>)"
-    using pda.stepn_steps[OF pda_stack_to_final] by fastforce
+    using pda.stepn_steps[OF pda_stack_to_final] by (fastforce simp add: stack_to_final_pda_def)
   then obtain n' where "n = Suc (Suc n')"
-    using stack_to_final_pda_path_length Suc_less_eq2 numeral_2_eq_2 by fastforce
+    using stack_to_final_pda_path_length by blast
   with stepn obtain p where "pda.stepn stack_to_final_pda n' (Old_st (init_state M), w, [Old_sym (init_symbol M), New_sym])
                                                                 (Old_st p, [], [New_sym])"
     using stack_to_final_pda_split_path by blast
   hence "pda.stepn M n' (init_state M, w, [(init_symbol M)]) (p, [], [])"
     using stack_to_final_pda_stepn by simp
-  thus "\<exists>q. pda.steps M (init_state M, w, [init_symbol M]) (q, [], [])"
+  thus ?l
     using stepn_steps by blast
 qed
 
